update

keyCert.v
@@ -1,7 +1,37 @@
 
-  Require Import Coq.Init.Nat.
-  Require Import Coq.Lists.List.
-  Import ListNotations.
+Require Import Coq.Init.Nat.
+Require Import Coq.Lists.List.
+Import ListNotations.
+
+
+
+
+Class DecEq (A : Type) := 
+{
+  decEq : forall x1 x2 : A, {x1 = x2} + {x1 <> x2}
+}.
+
+Ltac fdeq :=
+  eauto; intros HC; inversion HC; congruence.
+
+Ltac ddeq :=
+  econstructor;
+  match goal with
+  | |- forall x1 x2 : _,_ =>
+      destruct x1, x2; eauto;
+      try right; fdeq
+  end.
+
+Ltac ideq :=
+  econstructor;
+  match goal with
+  | |- forall x1 x2 : _,_ =>
+      induction x1 as [|x1 IHx1]; destruct x2;
+      try destruct (IHx1 x2); eauto
+  end.
+
+
+
 
 
 
@@ -12,78 +42,219 @@
 
 
 (* Each key pair has a unique identifier *)
-  Definition key_id := nat.
+Definition keyIdType := nat.
 
 
-(* Attributes relevant to this specification *)
+(* TPM key attributes relevant to this specification *)
 
-  Inductive restrict_att : Type :=
-  | Restricted
-  | NonRestricted.
+Inductive Restricted : Type :=
+| Restricting
+| NonRestricting.
 
-  Inductive sign_att : Type :=
-  | Signing
-  | NonSigning.
+Inductive Sign : Type :=
+| Signing
+| NonSigning.
 
-  Inductive decrypt_att : Type :=
-  | Decrypting
-  | NonDecrypting.
+Inductive Decrypt : Type :=
+| Decrypting
+| NonDecrypting.
+
+Inductive FixedTPM : Type :=
+| Fixing
+| NonFixing.
+
 
 
 (* Key pair definitions *)
 
-  Inductive pubKey : Type :=
-  | Public : key_id -> restrict_att -> sign_att -> decrypt_att -> pubKey.
+Inductive pubKey : Type :=
+| Public : keyIdType -> Restricted -> Sign -> Decrypt -> FixedTPM -> pubKey.
 
-  Inductive privKey : Type :=
-  | Private : key_id -> restrict_att -> sign_att -> decrypt_att -> privKey.
+Inductive privKey : Type :=
+| Private : keyIdType -> Restricted -> Sign -> Decrypt -> FixedTPM -> privKey.
 
 
 (* Functions to get a key's inverse *)
 
-  Definition pubtoPrivKey (k : pubKey) : privKey :=
-    match k with
-    | Public i r s d => Private i r s d
-    end.
+Definition pubToPrivKey (k : pubKey) : privKey :=
+  match k with
+  | Public i r s d f => Private i r s d f
+  end.
 
-  Definition privToPubKey (k : privKey) : pubKey :=
-    match k with
-    | Private i r s d => Public i r s d
-    end.
+Definition privToPubKey (k : privKey) : pubKey :=
+  match k with
+  | Private i r s d f => Public i r s d f
+  end.
 
 
 (* Attribute requirements for EK, AK, DevID, and CA keys *)
 
-  Definition endorsementKey (k : pubKey) : Prop :=
-    match k with
-    | Public _ Restricted NonSigning Decrypting => True
-    | _ => False
-    end.
+Definition endorsementKey (k : pubKey) : Prop :=
+  match k with
+  | Public _ Restricting NonSigning Decrypting Fixing => True
+  | _ => False
+  end.
 
-  Definition attestationKey (k : pubKey) : Prop :=
-    match k with
-    | Public _ Restricted Signing NonDecrypting => True
-    | _ => False
-    end.
+Definition attestationKey (k : pubKey) : Prop :=
+  match k with
+  | Public _ Restricting Signing NonDecrypting Fixing => True
+  | _ => False
+  end.
 
-  Definition devidKey (k : pubKey) : Prop :=
-    match k with
-    | Public _ NonRestricted Signing NonDecrypting => True
-    | _ => False
-    end.
+Definition devidKey (k : pubKey) : Prop :=
+  match k with
+  | Public _ NonRestricting Signing NonDecrypting Fixing => True
+  | _ => False
+  end.
 
-  Definition caKey (k : pubKey) : Prop :=
-    match k with
-    | Public _ NonRestricted Signing _ => True
-    | _ => False
-    end.
+Definition caKey (k : pubKey) : Prop :=
+  match k with
+  | Public _ NonRestricting Signing NonDecrypting Fixing => True
+  | _ => False
+  end.
 
-(* Roles in this specification *)
-(* Currently unused. Should include adversary? *)
-  Inductive entity : Set :=
-  | tm
-  | oem
-  | owner.
+
+
+(* Decidable equality of keys *)
+Local Instance decEq_keyID : DecEq keyIdType.
+  ideq.
+Qed.
+
+Local Instance decEq_Restricted : DecEq Restricted.
+  ddeq.
+Qed.
+  
+Local Instance decEq_Sign : DecEq Sign.
+  ddeq.
+Qed.
+
+Local Instance decEq_Decrypt : DecEq Decrypt.
+  ddeq.
+Qed.
+
+Local Instance decEq_FixedTPM : DecEq FixedTPM.
+  ddeq.
+Qed.
+
+Local Instance decEq_pubKey : DecEq pubKey.
+  econstructor; induction x1; destruct x2;
+  destruct (decEq k k0);
+  destruct (decEq r r0);
+  destruct (decEq s s0);
+  destruct (decEq d d0);
+  destruct (decEq f f0);
+  subst; eauto; right; fdeq.
+Qed.
+
+Local Instance decEq_privKey : DecEq privKey.
+  econstructor; induction x1; destruct x2.
+  destruct (decEq k k0); 
+  destruct (decEq r r0);
+  destruct (decEq s s0); 
+  destruct (decEq d d0);
+  destruct (decEq f f0);
+  subst; eauto; right; fdeq.
+Qed.
+
+
+
+
+
+
+
+
+
+
+
+
+
+
+
+
+
+
+
+
+
+
+(* Messages *)
+(* ******** *)
+
+
+(* Arbitrary type to model identifying information *)
+Definition tpmInfoType := nat.
+Definition deviceInfoType := nat.
+
+Inductive identifier : Type :=
+| TPM_info : tpmInfoType -> identifier
+| Device_info : deviceInfoType -> identifier.
+
+
+Inductive signedCert : Type :=
+| Cert : pubKey -> identifier -> privKey -> signedCert.
+
+
+(* Arbitrary type to model random numbers *)
+Definition randType := nat.
+
+
+(* Messages includes all structures required in this specification *)
+Inductive message : Type :=
+| publicKey : pubKey -> message
+| privateKey : privKey -> message
+| hash : message -> message
+| signature : message -> privKey -> message
+| TPM2B_Attest : pubKey -> message
+| encryptedCredential : message -> randType -> pubKey -> message
+| randomNum : randType -> message
+| TCG_CSR_IDevID : identifier -> signedCert -> pubKey -> message
+| TCG_CSR_LDevID : message -> signedCert -> message
+| signedCertificate : signedCert -> message
+| pair : message -> message -> message.
+
+
+(* Decidable equality of messages *)
+
+Local Instance decEq_identifier : DecEq identifier.
+  econstructor; induction x1; destruct x2; try (right; fdeq);
+  try destruct (decEq t t0);
+  try destruct (decEq d d0);
+  subst; eauto; right; fdeq.
+Qed.
+
+Local Instance decEq_signedCert : DecEq signedCert.
+  econstructor; destruct x1, x2;
+  destruct (decEq p p1); 
+  destruct (decEq i i0); 
+  destruct (decEq p0 p2);
+  subst; eauto; right; fdeq.
+Qed.
+
+Local Instance decEq_randType : DecEq randType.
+  ideq.
+Qed.
+
+Local Instance decEq_message : DecEq message.
+  econstructor; induction x1; destruct x2; try (right; fdeq);
+  try destruct (decEq p p0);
+  try destruct (decEq r r0);
+  try destruct (decEq i i0);
+  try destruct (decEq s s0);
+  try destruct (IHx1 x2);
+  subst; eauto; try (right; fdeq).
+  destruct (IHx1_1 x2_1);
+  destruct (IHx1_2 x2_2);
+  subst; eauto; right; fdeq.
+Qed.
+
+
+
+
+
+
+
+
+
 
 
 
@@ -91,57 +262,68 @@
 (* ******** *)
 
 
-(* Arbitrary type to model random numbers *)
-  Definition randType := nat.
-
-(* Messages includes all structures required in this specification *)
-  Inductive message : Type :=
-  | publicKey : pubKey -> message
-  | privateKey : privKey -> message
-  | rand : randType -> message
-  | hash : message -> message
-  | sign : message -> privKey -> message
-  | TPM2B_Attest : pubKey -> message
-  | credential : message -> randType -> message
-  | encrypt : message -> pubKey -> message
-  | TCG_CSR_IDevID : message -> pubKey -> message
-  | TCG_CSR_LDevID : message -> message -> message
-  | certificate : pubKey -> message    (* TODO: pubKey -> id -> message *)
-  | pair : message -> message -> message.
-
-
 (* Includes both TPM and non-TPM commands required in this specification *)
-  Inductive command : Type :=
-  | CheckAttributes : pubKey -> restrict_att -> sign_att -> decrypt_att -> command
-  | TPM2_GetRandom : randType -> command
-  | CheckNonce : message -> randType -> command
-  | TPM2_Hash : message -> command
-  | CheckHash : message -> message -> command
-  | TPM2_Sign : message -> privKey -> command
-  | CheckSig : message -> pubKey -> command
-  | TPM2_Certify : pubKey -> privKey -> command
-  | TPM2_MakeCredential : message -> randType -> pubKey -> command
-  | TPM2_ActivateCredential : message -> privKey -> privKey -> command
-  | MakeCSR_IDevID : message -> pubKey -> command
-  | MakeCSR_LDevID : message -> message -> command
-  | MakeCert : pubKey -> privKey -> command  (* TODO: pubKey -> id -> privKey -> message *)
-  | CheckCert : message -> pubKey -> command
-  | Sequence : command -> command -> command.
+Inductive command : Type :=
+| TPM2_Hash : message -> command
+| CheckHash : message -> message -> command
+| TPM2_Sign : message -> privKey -> command
+| TPM2_Certify : pubKey -> privKey -> command
+| CheckSig : message -> pubKey -> command
+| TPM2_MakeCredential : message -> randType -> pubKey -> command
+| TPM2_ActivateCredential : message -> privKey -> privKey -> command
+| MakeCSR_IDevID : identifier -> signedCert -> pubKey -> command
+| MakeCSR_LDevID : message -> signedCert -> command
+| CheckCert : signedCert -> pubKey -> command
+| CheckAttributes : pubKey -> Restricted -> Sign -> Decrypt -> FixedTPM -> command
+| MakePair : message -> message -> command.
 
 
 (* State corresponds to what an entity knows *)
-(* Not necessarily exhaustive *)
-  Definition state := list message.
+(* States are treated as sets *)
 
+Definition state := list message.
 
-(* TPM State contains everything produced by a TPM command *)
+(* TPM State isSuperseqOf everything produced by a TPM command *)
 (* Subset of the general state *)
-  Definition tpm_state := list message.
+Definition tpm_state := list message.
 
 
-(* Notations for pairs of messages and sequences of commands *)
-  Notation "m1 ,, m2" := (pair m1 m2)  (at level 90, left associativity).
-  Notation "c1 ;; c2" := (Sequence c1 c2) (at level 90, left associativity).
+(* Set inclusion over states *)
+
+Definition Included (st1 st2 : list message) : Prop := forall m,
+In m st1 ->
+In m st2.
+
+Notation "st1 \subsetOf st2" := (Included st1 st2) (at level 92, left associativity).
+
+Lemma Included_transitive : forall st1 st2 st3,
+  st1 \subsetOf st2 ->
+  st2 \subsetOf st3 ->
+  st1 \subsetOf st3.
+Proof.
+  intros st1 st2 st3 H12 H23; intros m' I; 
+  apply H23; apply H12; assumption.
+Qed.
+
+
+
+
+(* Decidable equality of commands *)
+Local Instance decEq_command : DecEq command.
+  econstructor; induction x1; destruct x2; try (right; fdeq);
+  try destruct (decEq p p0);
+  try destruct (decEq r r0);
+  try destruct (decEq s s0);
+  try destruct (decEq d d0);
+  try destruct (decEq f f0);
+  try destruct (decEq m m0);
+  try destruct (decEq i i0);
+  try (destruct (decEq m m1); destruct (decEq m0 m2));
+  try (destruct (decEq p p1); destruct (decEq p0 p2));
+  subst; eauto; right; fdeq.
+Qed.
+
+
 
 
 
@@ -151,74 +333,24 @@
 (* ********************* *)
 
 
-(* Inductive proposition describing command execution *)
+(* Inductive proposition describing individual command execution *)
+(* Relates an initial state, a command, and a final state *)
   Inductive execute : tpm_state * state -> command -> tpm_state * state -> Prop :=
-(*
-  CheckAttributes
-  ***************
-  Inputs: 
-    Public Key
-    Attributes
-  Success Conditions:
-    Public Key has all Attributes
-  Updates to State:
-    None
-*)
-  | E_CheckAttributes : forall stTPM st i r s d,
-      execute (stTPM, st)
-              (CheckAttributes (Public i r s d) r s d)
-              (stTPM,
-               st)
-(*
-  TPM2_GetRandom
-  **************
-  Inputs: 
-    Random Number
-  Success Conditions:
-    None
-  Updates to State:
-    Random Number to TPM State
-*)
-  | E_GetRandom : forall stTPM st g,
-      execute 
-        (stTPM, st)
-        (TPM2_GetRandom g)
-        (rand g :: stTPM,
-         rand g :: st)
-(*
-  CheckNonce
-  **********
-  Inputs: 
-    Random Number
-    Golden Value
-  Success Conditions:
-    Golden Value resides in TPM
-    Random Number is Golden Value
-  Updates to State:
-    None
-*)
-  | E_CheckNonce : forall stTPM st g,
-      In (rand g) stTPM ->
-      execute (stTPM, st)
-              (CheckNonce (rand g) g)
-              (stTPM,
-               st)
 (*
   TPM2_Hash
   *********
   Inputs: 
     Message
   Success Conditions:
-    None
+    Message is in state
   Updates to State:
-    The hash of Message to TPM State
+    hash of Message to TPM State
 *)
-  | E_Hash : forall stTPM st m,
-      In m st ->
-      execute (stTPM, st)
-              (TPM2_Hash m)
-              (hash m :: stTPM,
-               hash m :: st)
+| E_Hash : forall stTPM st m,
+    In m st ->
+    execute (stTPM, st)
+            (TPM2_Hash m)
+            (hash m :: stTPM, hash m :: st)
 (*
   CheckHash
   *********
@@ -232,53 +364,69 @@
   Updates to State:
     None
 *)
-  | E_CheckHash : forall stTPM st m,
-      In (hash m) st ->
-      In m st ->
-      execute (stTPM, st)
-              (CheckHash (hash m) m)
-              (stTPM,
-               st)
+| E_CheckHash : forall stTPM st m,
+    In (hash m) st ->
+    In m st ->
+    execute (stTPM, st)
+            (CheckHash (hash m) m)
+            (stTPM, st)
 (*
-  TPM2_Sign
-  *********
+  TPM2_Sign Restricted
+  ********************
   Inputs: 
     Message
     Private Key
   Success Conditions:
     Private Key resides in TPM
     Message resides in TPM
-    Private Key has Restricted and Signing attributes
+    Private Key has Restricting and Signing attributes
   Updates to State:
-    Message signed by Private Key to TPM State
+    Message signed by Private Key
 *)
-  | E_SignR : forall stTPM st m i d,
-      In (privateKey (Private i Restricted Signing d)) stTPM ->
-      In m stTPM ->
-      execute (stTPM,st)
-              (TPM2_Sign m (Private i Restricted Signing d))
-              (sign m (Private i Restricted Signing d) :: stTPM,
-               sign m (Private i Restricted Signing d) :: st)
+| E_SignR : forall stTPM st m i d f,
+    In (privateKey (Private i Restricting Signing d f)) stTPM ->
+    In m stTPM ->
+    execute (stTPM,st)
+            (TPM2_Sign m (Private i Restricting Signing d f))
+            (stTPM, signature m (Private i Restricting Signing d f) :: st)
 (*
-  TPM2_Sign
-  *********
+  TPM2_Sign Not-Restricted
+  ************************
   Inputs: 
     Message
     Private Key
   Success Conditions:
     Private Key resides in TPM
     Message is in state
-    Private Key has NonRestricted and Signing attributes
+    Private Key has NonRestricting and Signing attributes
   Updates to State:
-    Message signed by Private Key to TPM State
+    Message signed by Private Key
 *)
-  | E_SignNR : forall stTPM st m i d,
-      In (privateKey (Private i NonRestricted Signing d)) stTPM ->
-      In m st ->
-      execute (stTPM, st)
-              (TPM2_Sign m (Private i NonRestricted Signing d))
-              (sign m (Private i NonRestricted Signing d) :: stTPM,
-               sign m (Private i NonRestricted Signing d) :: st)
+| E_SignNR : forall stTPM st m i d f,
+    In (privateKey (Private i NonRestricting Signing d f)) stTPM ->
+    In m st ->
+    execute (stTPM, st)
+            (TPM2_Sign m (Private i NonRestricting Signing d f))
+            (stTPM, signature m (Private i NonRestricting Signing d f) :: st)
+(*
+  TPM2_Certify
+  ************
+  Inputs: 
+    Public Key
+    Private Key
+  Success Conditions:
+    The inverse of Public Key resides in TPM
+    Private Key resides in TPM
+    Private Key has Signing attribute
+  Updates to State:
+    TPM2B_Attest structure of Public Key signed by Private Key
+*)
+| E_Certify : forall stTPM st i r s d f i0 r0 d0 f0,
+    In (privateKey (Private i r s d f)) stTPM -> 
+    In (privateKey (Private i0 r0 Signing d0 f0)) stTPM ->
+    execute (stTPM, st)
+            (TPM2_Certify (Public i r s d f) (Private i0 r0 Signing d0 f0))
+            (stTPM, signature (TPM2B_Attest (Public i r s d f)) (Private i0 r0 Signing d0 f0) :: st)
 (*
   CheckSig
   ********
@@ -292,60 +440,39 @@
   Updates to State:
     None
 *)
-  | E_CheckSig : forall stTPM st m i r s d,
-      In (sign m (Private i r s d)) st ->
-      In (publicKey (Public i r s d)) st ->
-      execute (stTPM, st)
-              (CheckSig (sign m (Private i r s d)) (Public i r s d))
-              (stTPM,
-               st)
-(*
-  TPM2_Certify
-  ************
-  Inputs: 
-    Public Key
-    Private Key
-  Success Conditions:
-    The inverse of Public Key resides in TPM
-    Private Key resides in TPM
-    Private Key has Signing attribute
-  Updates to State:
-    TPM2B_Attest structure of Public Key signed by Private Key to TPM State
-*)
-  | E_Certify : forall stTPM st i r s d i0 r0 d0,
-      In (privateKey (Private i r s d)) stTPM -> 
-      In (privateKey (Private i0 r0 Signing d0)) stTPM ->
-      execute (stTPM, st)
-              (TPM2_Certify (Public i r s d) (Private i0 r0 Signing d0))
-              (sign (TPM2B_Attest (Public i r s d)) (Private i0 r0 Signing d0) :: stTPM,
-               sign (TPM2B_Attest (Public i r s d)) (Private i0 r0 Signing d0) :: st)
+| E_CheckSig : forall stTPM st m i r s d f,
+    In (signature m (Private i r s d f)) st ->
+    In (publicKey (Public i r s d f)) st ->
+    execute (stTPM, st)
+            (CheckSig (signature m (Private i r s d f)) (Public i r s d f))
+            (stTPM, st)
 (*
   TPM2_MakeCredential
   *******************
-  Inputs: 
-    Message
+  Inputs:
+    Name
     Random Number
     Public Key
   Success Conditions:
-    Message in in state
-    Random Number resides in TPM
-    Public Key has Decrypting attribute
+    Name is in state
+    Random Number is in state
+    Public Key is in state
+    Public Key is an endorsement key
   Updates to State:
-    Credential structure of Message and Random Number encrypted with Public Key to TPM State
+    credential containing Name and Random Number encrypted by Public Key
 *)
-  | E_MakeCredential : forall stTPM st m g i r s,
-      In m st ->
-      In (rand g) stTPM ->
-      In (publicKey (Public i r s Decrypting)) st ->
-      execute (stTPM, st)
-              (TPM2_MakeCredential m g (Public i r s Decrypting)) 
-              (encrypt (credential m g) (Public i r s Decrypting) :: stTPM,
-               encrypt (credential m g) (Public i r s Decrypting) :: st)
+| E_MakeCredential : forall stTPM st n g i,
+    In n st ->
+    In (randomNum g) st ->
+    In (publicKey (Public i Restricting NonSigning Decrypting Fixing)) st ->
+    execute (stTPM, st)
+            (TPM2_MakeCredential n g (Public i Restricting NonSigning Decrypting Fixing))
+            (stTPM, encryptedCredential n g (Public i Restricting NonSigning Decrypting Fixing) :: st)
 (*
   TPM2_ActivateCredential
   ***********************
   Inputs: 
-    Encrypted Credential (Credential contains Message and Random Number)
+    Encrypted Credential (isSuperseqOf Name and Random Number)
     Private Key A
     Private Key B
   Success Conditions:
@@ -353,237 +480,1200 @@
     Private Key A resides in TPM
     Private Key B resides in TPM
     Private Key A is the inverse of the key that created Encrypted Credential
-    Message is the hash of the inverse of Private Key B
+    Name is the hash of the inverse of Private Key B
   Updates to State:
-    Random Number and Credential to TPM State
+    Random Number
 *)
-  | E_ActivateCredential : forall stTPM st m g i r s d i0 r0 s0 d0,
-      In (encrypt (credential m g) (Public i r s d)) st ->
-      In (privateKey (Private i r s d)) stTPM ->
-      In (privateKey (Private i0 r0 s0 d0)) stTPM ->
-      execute (stTPM, m::st) (CheckHash m (publicKey (Public i0 r0 s0 d0))) (stTPM, m::st) ->
-      execute (stTPM, st)
-              (TPM2_ActivateCredential (encrypt (credential m g) (Public i r s d)) 
-                                      (Private i r s d)
-                                      (Private i0 r0 s0 d0)) 
-              (rand g :: credential m g :: stTPM,
-               rand g :: credential m g :: st)
+| E_ActivateCredential : forall stTPM st n g i r s d f i0 r0 s0 d0 f0,
+    In (encryptedCredential n g (Public i r s d f)) st ->
+    In (privateKey (Private i r s d f)) stTPM ->
+    In (privateKey (Private i0 r0 s0 d0 f0)) stTPM ->
+    execute (stTPM, n::st) (CheckHash n (publicKey (Public i0 r0 s0 d0 f0))) (stTPM, n::st) ->
+    execute (stTPM, st)
+            (TPM2_ActivateCredential (encryptedCredential n g (Public i r s d f)) 
+                                     (Private i r s d f)
+                                     (Private i0 r0 s0 d0 f0)) 
+            (stTPM, randomNum g :: st)
+
+
 (*
   MakeCSR_IDevID
   **************
   Inputs: 
-    Message
+    Identifier
+    Certificate
     Public Key
   Success Conditions:
-    Message is in state
+    Certificate is in state
     Public Key is in state
   Updates to State:
-    TCG_CSR_IDevID of Message and Public Key to State
+    TCG_CSR_IDevID containing Identifier, Certificate, and Public Key
 *)
-  | E_MakeCSR_IDevID : forall stTPM st m i r s d,
-      In m st ->
-      In (publicKey (Public i r s d)) st ->
-      execute (stTPM, st)
-              (MakeCSR_IDevID m (Public i r s d))
-              (stTPM,
-               TCG_CSR_IDevID m (Public i r s d) :: st)
+| E_MakeCSR_IDevID : forall stTPM st id crt k,
+    In (signedCertificate crt) st ->
+    In (publicKey k) st ->
+    execute (stTPM, st)
+            (MakeCSR_IDevID id crt k)
+            (stTPM, TCG_CSR_IDevID id crt k :: st)
 (*
   MakeCSR_LDevID
   **************
   Inputs: 
+    Message
+    Certificate
+  Success Conditions:
+    Message is in state
+    Certificate is in state
+  Updates to State:
+    TCG_CSR_LDevID containing Message and Certificate
+*)
+| E_MakeCSR_LDevID : forall stTPM st m crt,
+    In m st ->
+    In (signedCertificate crt) st ->
+    execute (stTPM, st)
+            (MakeCSR_LDevID m crt)
+            (stTPM, TCG_CSR_LDevID m crt :: st)
+(*
+  CheckCert
+  *********
+  Inputs: 
+    Signed Certificate
+    Public Key
+  Success Conditions:
+    Signed Certificate is in state
+    Public Key is in state
+    Public Key is the inverse of the key that created Signed Certificate
+  Updates to State:
+    None
+*)
+| E_CheckCert : forall stTPM st k id i r s d f,
+    In (signedCertificate (Cert k id (Private i r s d f))) st ->
+    In (publicKey (Public i r s d f)) st ->
+    execute (stTPM, st)
+            (CheckCert (Cert k id (Private i r s d f)) (Public i r s d f))
+            (stTPM, st)
+(*
+  CheckAttributes
+  ***************
+  Inputs: 
+    Public Key
+    Attributes
+  Success Conditions:
+    Public Key is in state
+    Public Key has all Attributes
+  Updates to State:
+    None
+*)
+| E_CheckAttributes : forall stTPM st i r s d f,
+    In (publicKey (Public i r s d f)) st ->
+    execute (stTPM, st)
+            (CheckAttributes (Public i r s d f) r s d f)
+            (stTPM, st)
+(*
+  MakePair
+  ********
+  Inputs:
     Message A
     Message B
   Success Conditions:
     Message A is in state
     Message B is in state
   Updates to State:
-    TCG_CSR_LDevID of Message A and Message B to State
-*)
-  | E_MakeCSR_LDevID : forall stTPM st m1 m2,
-      In m1 st ->
-      In m2 st ->
-      execute (stTPM, st)
-              (MakeCSR_LDevID m1 m2)
-              (stTPM,
-               TCG_CSR_LDevID m1 m2 :: st)
-(*
-  MakeCert
-  ********
-  Inputs: 
-    Public Key
-    Private Key
-  Success Conditions:
-    Public Key is in state
-    Private Key resides in TPM
-    Private Key has NonRestricted and Signing attributes
-  Updates to State:
-    Certificate of Public Key signed by Private Key to TPM State
-*)
-  | E_MakeCert : forall stTPM st i r s d i0 d0,
-      In (publicKey (Public i r s d)) st ->
-      In (privateKey (Private i0 NonRestricted Signing d0)) stTPM ->
-      execute (stTPM, st)
-              (MakeCert (Public i r s d) (Private i0 NonRestricted Signing d0))
-              (sign (certificate (Public i r s d)) (Private i0 NonRestricted Signing d0) :: stTPM,
-               sign (certificate (Public i r s d)) (Private i0 NonRestricted Signing d0) :: st)
-(*
-  CheckCert
-  *********
-  Inputs: 
-    Signature
-    Public Key
-  Success Conditions:
-    Signature is in state
-    Public Key is in state
-    Signature contains Certificate
-    Public Key is the inverse of the key that created Signature
-  Updates to State:
-    None
-*)
-  | E_CheckCert : forall stTPM st k i r s d,
-      In (sign (certificate k) (Private i r s d)) st ->
-      In (publicKey (Public i r s d)) st ->
-      execute (stTPM, st)
-              (CheckCert (sign (certificate k) (Private i r s d)) (Public i r s d))
-              (stTPM,
-              st)
-(*
-  Sequence
-  ********
-  Inputs: 
-    Command A
-    Command B
-  Success Conditions:
-    None
-  Updates to State:
-    Effects from Command A and Command B
-*)
-  | E_Sequence : forall ini mid fin c1 c2,
-      execute ini c1 mid ->
-      execute mid c2 fin ->
-      execute ini (Sequence c1 c2) fin.
+    pair containing Message A and Message B *)
+| E_MakePair : forall stTPM st m1 m2,
+    In m1 st ->
+    In m2 st ->
+    execute (stTPM, st)
+            (MakePair m1 m2)
+            (stTPM, pair m1 m2 :: st).
 
 
-(* Execute relation is a partial function *)
-  Theorem execute_deterministic : forall ini c fin1 fin2,
-    execute ini c fin1 ->
-    execute ini c fin2 ->
-    fin1 = fin2.
-  Proof.
-    intros ini c fin1 fin2 E1 E2.
-    generalize dependent fin2.
-    induction E1; intros fin2 E2; inversion E2; subst; try reflexivity.
-    assert (mid = mid0) as EQ_mid.
-    - apply IHE1_1; assumption.
-    - apply IHE1_2; rewrite EQ_mid; assumption.
-  Qed.
+Lemma exec_deterministic : forall ini c fin1 fin2,
+  execute ini c fin1 ->
+  execute ini c fin2 ->
+  fin1 = fin2.
+Proof.
+  intros ini c fin1 fin2 E1 E2;
+  destruct E1; inversion E2; subst; reflexivity.
+Qed.
+
+Lemma exec_expansion : forall iniTPM ini c finTPM fin,
+  execute (iniTPM,ini) c (finTPM,fin) ->
+  (iniTPM \subsetOf finTPM) /\
+  (ini \subsetOf fin).
+Proof.
+  intros iniTPM ini c finTPM fin E; split;
+  destruct c; inversion E; subst; 
+  intros m' I; try (repeat apply in_cons); assumption.
+Qed.
+
+Lemma exec_cannotGenerateKey : forall c iniTPM ini finTPM fin k,
+  execute (iniTPM, ini) c (finTPM, fin) ->
+  In (privateKey k) finTPM ->
+  In (privateKey k) iniTPM.
+Proof.
+  destruct c; intros iniTPM ini finTPM fin k E I;
+  inversion E; subst; try inversion I as [EQ_false | I']; 
+  try inversion EQ_false; assumption.
+Qed.
+
+Lemma exec_cannotGenerateRand_contrapositive : forall c iniTPM ini finTPM fin g,
+  execute (iniTPM, ini) c (finTPM, fin) ->
+  ~ In (randomNum g) ini ->
+  (forall n k, ~ In (encryptedCredential n g k) ini) ->
+  ~ In (randomNum g) fin.
+Proof.
+  induction c; intros iniTPM ini finTPM fin g E Ng N;
+  inversion E; subst; try assumption;
+  intros HC; inversion HC; try inversion H; subst; try congruence;
+  destruct (N n (Public i r s d f)); assumption.
+Qed.
 
 
-  Ltac execute_constructor :=
-    match goal with
-    | [ |- execute _ (Sequence _ _) _ ] => eapply E_Sequence
-    | [ |- execute _ _ _] => constructor
-    end.
-
-
-  Lemma sequence_split : forall ini c1 c2 fin,
-    execute ini (c1 ;; c2) fin ->
-    exists mid, (execute ini c1 mid /\ execute mid c2 fin).
-  Proof.
-    intros ini c1 c2 fin H; inversion H; subst.
-    exists mid; split; assumption.
-  Qed.
+Lemma exec_cannotGenerateCred_contrapositive : forall c iniTPM ini finTPM fin n g k,
+  execute (iniTPM, ini) c (finTPM, fin) ->
+  ~ In (encryptedCredential n g k) ini ->
+  ~ In (randomNum g) ini ->
+  ~ In (encryptedCredential n g k) fin.
+Proof.
+  induction c;  intros iniTPM ini finTPM fin n g k E Ne N;
+  inversion E; subst; try assumption;
+  intros HC; inversion HC; try inversion H; congruence.
+Qed.
 
 
 
 
-(* Message Discovery *)
+
+
+
+
+
+
+
+
+
+(* Execution of Sequences of Commands *)
+(* ********************************** *)
+
+
+Inductive sequence : Type :=
+| Sequence : command -> sequence -> sequence
+| Done : sequence.
+
+Infix ";;" := Sequence (at level 60, right associativity).
+
+Fixpoint command_in_sequence (cmd : command) (seq : sequence)  :=
+  match seq with
+  | c ;; s =>
+      if (decEq cmd c)
+      then True
+      else command_in_sequence cmd s
+  | Done => False
+  end.
+
+Inductive seq_execute : tpm_state * state -> sequence -> tpm_state * state -> Prop :=
+| SE_Seq : forall ini mid fin c s,
+    execute ini c mid ->
+    seq_execute mid s fin ->
+    seq_execute ini (Sequence c s) fin
+| SE_Done : forall ini,
+    seq_execute ini Done ini.
+
+(* Sequential execution relation is a partial function *)
+Theorem seq_exec_deterministic : forall ini s fin1 fin2,
+  seq_execute ini s fin1 ->
+  seq_execute ini s fin2 ->
+  fin1 = fin2.
+Proof.
+  intros ini s fin1 fin2 E1 E2; generalize dependent fin2;
+  induction E1; intros fin2 E2; inversion E2; subst.
+  - assert (mid = mid0) as EQ_mid;
+    [ apply exec_deterministic with (ini := ini) (c := c)
+    | apply IHE1; rewrite <- EQ_mid in H5 ]; assumption.
+  - reflexivity.
+Qed.
+
+(* Sequential execution does not remove elements from the state *)
+Theorem seq_exec_expansion : forall iniTPM ini s finTPM fin,
+  seq_execute (iniTPM,ini) s (finTPM,fin) ->
+  (iniTPM \subsetOf finTPM) /\ (ini \subsetOf fin).
+Proof.
+  intros iniTPM ini s finTPM fin E; split;
+  generalize dependent fin; generalize dependent finTPM;
+  generalize dependent ini; generalize dependent iniTPM;
+  induction s; intros;
+  inversion E; subst; try (intros m' I; assumption);
+  destruct mid as [midTPM mid];
+  assert (Inc : (iniTPM \subsetOf midTPM) /\ (ini \subsetOf mid)); 
+  try (apply exec_expansion with (c := c); assumption).
+  - apply Included_transitive with (st2 := midTPM);
+    [ apply Inc
+    | apply IHs with (ini := mid) (fin := fin); assumption ].
+  - apply Included_transitive with (st2 := mid);
+    [ apply Inc
+    | apply IHs with (iniTPM := midTPM) (finTPM := finTPM); assumption ].
+Qed.
+
+(* Sequential execution cannot add a key to the state *)
+Theorem seq_exec_cannotGenerateKey : forall s iniTPM ini finTPM fin k,
+  seq_execute (iniTPM, ini) s (finTPM, fin) ->
+  In (privateKey k) finTPM ->
+  In (privateKey k) iniTPM.
+Proof.
+  induction s; intros iniTPM ini finTPM fin k E I;
+  inversion E; subst; try assumption; destruct mid as [midTPM mid];
+  eapply exec_cannotGenerateKey; eauto.
+Qed.
+
+
+(* Sequential execution cannot add a random number to the state without an encrypted credential *)
+Theorem seq_exec_cannotGenerateRand_contrapositive : forall s iniTPM ini finTPM fin g,
+  seq_execute (iniTPM, ini) s (finTPM, fin) ->
+  ~ In (randomNum g) ini ->
+  (forall n k, ~ In (encryptedCredential n g k) ini) ->
+  ~ In (randomNum g) fin.
+Proof.
+  induction s; intros iniTPM ini finTPM fin g E Ng N.
+  - destruct c; inversion E; inversion H2; 
+    subst; eapply IHs; try fdeq;
+    try (intros n0 k HC; inversion HC; try congruence; destruct (N n0 k); assumption);
+    intros HC; inversion HC;
+    [ inversion H; subst; destruct (N n (Public i r s1 d f)); assumption
+    | congruence ].
+  - inversion E; subst; congruence.
+Qed.
+
+
+(* Sequential execution cannot add an encrypted credential to the state without a random number *)
+Theorem seq_exec_cannotGenerateCred_contrapositive : forall s iniTPM ini finTPM fin n g k,
+  seq_execute (iniTPM, ini) s (finTPM, fin) ->
+  (forall n k, ~ In (encryptedCredential n g k) ini) ->
+  ~ In (randomNum g) ini ->
+  ~ In (encryptedCredential n g k) fin.
+Proof.
+  induction s; intros iniTPM ini finTPM fin n g k E Ne N;
+  inversion E; subst; 
+  [ destruct mid as [midTPM mid]; eapply IHs; eauto
+  | intros HC; destruct (Ne n k); assumption];
+  [ intros n0 k0; eapply exec_cannotGenerateCred_contrapositive; eauto
+  | eapply exec_cannotGenerateRand_contrapositive; eauto].
+Qed.
+
+
+
+
+
+
+
+
+
+
+
+(* Message Inference *)
 (* ***************** *)
 
-(* An entity who knows a message can discover additional messages from it *)
-  Inductive discoverable : message -> state -> Prop :=
-  | D_publicKey : forall k,
-      discoverable (publicKey k) [publicKey k]
-  | D_privateKey : forall k,
-      discoverable (privateKey k) [privateKey k]
-  | D_rand : forall r,
-      discoverable (rand r) [rand r]
-  | D_hash : forall m,
-      discoverable (hash m) [hash m]
-  | D_sign : forall m k st,               (* contents of signature *)
-      discoverable m st ->
-      discoverable (sign m k) ((sign m k)::st)
-  | D_Attest : forall k,                  (* contents of TPM2_Attest structure *)
-      discoverable (TPM2B_Attest k) [(TPM2B_Attest k); (publicKey k)] 
-  | D_credential : forall m r,
-      discoverable (credential m r) [credential m r]
-  | D_encrypt : forall m k,
-      discoverable (encrypt m k) [encrypt m k]
-  | D_CSR_IDevID : forall m k st,         (* contents of TCG_CSR_IDevID *)
-      discoverable m st ->
-      discoverable (TCG_CSR_IDevID m k) ([(TCG_CSR_IDevID m k); (publicKey k)]++st)
-  | D_CSR_LDevID : forall m1 m2 st1 st2,  (* contents of TCG_CSR_LDevID *)
-      discoverable m1 st1 ->
-      discoverable m2 st2 ->
-      discoverable (TCG_CSR_LDevID m1 m2) ((TCG_CSR_LDevID m1 m2)::st1++st2)
-  | D_certificate : forall k,             (* contents of certificate *)
-      discoverable (certificate k) [(certificate k); (publicKey k)]
-  | D_pair : forall m1 m2 st1 st2,        (* contents of pair *)
-      discoverable m1 st1 ->
-      discoverable m2 st2 -> 
-      discoverable (pair m1 m2) ((m1,,m2)::(st1++st2)).
+
+Inductive inferrable : message -> state -> Prop :=
+| I_publicKey : forall k,
+    inferrable (publicKey k)
+               [publicKey k]
+| I_privateKey : forall k,
+    inferrable (privateKey k)
+               [privateKey k]
+| I_hash : forall m,
+    inferrable (hash m)
+               [hash m]
+| I_signature : forall m k st,
+    inferrable m st ->
+    inferrable (signature m k)
+               (signature m k :: st)
+| I_Attest : forall k,
+    inferrable (TPM2B_Attest k)
+               [TPM2B_Attest k ; publicKey k]
+| I_encryptedCredential : forall n g k,
+    inferrable (encryptedCredential n g k)
+               [encryptedCredential n g k]
+| I_randomNum : forall g,
+    inferrable (randomNum g)
+               [randomNum g]
+| I_CSR_IDevID : forall id crt k st,
+    inferrable (signedCertificate crt) st ->
+    inferrable (TCG_CSR_IDevID id crt k)
+               (TCG_CSR_IDevID id crt k :: publicKey k :: st)
+| I_CSR_LDevID : forall m crt st1 st2,
+    inferrable m st1 ->
+    inferrable (signedCertificate crt) st2 ->
+    inferrable (TCG_CSR_LDevID m crt) 
+               (TCG_CSR_LDevID m crt :: st1 ++ st2)
+| I_signedCertificate : forall k id k_ca,
+    inferrable (signedCertificate (Cert k id k_ca)) 
+               [signedCertificate (Cert k id k_ca) ; publicKey k]
+| I_pair : forall m1 m2 st1 st2,
+    inferrable m1 st1 ->
+    inferrable m2 st2 -> 
+    inferrable (pair m1 m2) 
+               (pair m1 m2 :: st1 ++ st2).
+
+Fixpoint inferFrom (msg : message) : state :=
+  match msg with
+  | signature m k => 
+      (signature m k :: inferFrom m)
+  | TPM2B_Attest k => 
+      [TPM2B_Attest k ; publicKey k]
+  | TCG_CSR_IDevID id (Cert k0 id0 k_ca) k => 
+      [TCG_CSR_IDevID id (Cert k0 id0 k_ca) k ; publicKey k ; 
+       signedCertificate (Cert k0 id0 k_ca) ; publicKey k0]
+  | TCG_CSR_LDevID m (Cert k id k_ca) => 
+      (TCG_CSR_LDevID m (Cert k id k_ca) :: inferFrom m ++ 
+      [signedCertificate (Cert k id k_ca) ; publicKey k])
+  | signedCertificate (Cert k id k_ca) => 
+      [signedCertificate (Cert k id k_ca) ; publicKey k]
+  | pair m1 m2 => 
+      (pair m1 m2 :: inferFrom m1 ++ inferFrom m2)
+  | _ => 
+      [msg]
+  end.
+
+(* inferFrom function and inferrable relation are equivalent *)
+Lemma inferFrom_iff_inferrable : forall m st,
+  inferFrom m = st <-> inferrable m st.
+Proof.
+  intros m st; split; intros H.
+  - generalize dependent m; assert (HI : forall m, inferrable m (inferFrom m)); intros m.
+  -- induction m; simpl; try destruct c; try destruct s; 
+     repeat constructor; assumption.
+  -- intros H; induction m; subst; apply HI.
+  - induction H; simpl; subst; try destruct crt; reflexivity.
+Qed.
 
 
-(* When sending a message the recipient can discover these additional messages *)
-  Fixpoint send (m : message) : state :=
+Fixpoint inferFromState (st : state) : state :=
+  match st with
+  | m :: st' => inferFrom m ++ inferFromState st'
+  | _ => st
+  end.
+  
+
+
+
+
+
+
+
+
+
+
+
+
+
+(* *************************** *)
+(* Key Certification Protocols *)
+(* *************************** *)
+(* *************************** *)
+
+
+
+
+(* Only public keys and certificates may reside in the initial state
+   of the Owner and OEM *)
+Definition needsGenerated (m : message) : Prop :=
   match m with
-    | sign m0 k => ((sign m0 k)::(send m0))
-    | TPM2B_Attest k => [(TPM2B_Attest k); (publicKey k)]
-    | TCG_CSR_IDevID m0 k => ([(TCG_CSR_IDevID m0 k); publicKey k]++(send m0))
-    | TCG_CSR_LDevID m1 m2 => ((TCG_CSR_LDevID m1 m2)::(send m1)++(send m2))
-    | certificate k => [(certificate k); (publicKey k)]
-    | pair m1 m2 => ((m1,,m2)::((send m1)++(send m2)))
-    | _ => [m]
+  | privateKey _ => True
+  | hash _ => True
+  | signature _ _ => True
+  | TPM2B_Attest _ => True
+  | encryptedCredential _ _ _ => True
+  | randomNum _ => True
+  | TCG_CSR_IDevID _ _ _ => True
+  | TCG_CSR_LDevID _ _ => True
+  | pair _ _ => True
+  | _ => False
+  end.
+
+
+(* Only private keys may reside in the initial TPM state
+   of the Owner and OEM *)
+Definition needsGeneratedTPM (m : message) : Prop :=
+  match m with
+  | publicKey _ => True
+  | hash _ => True
+  | signature _ _ => True
+  | TPM2B_Attest _ => True
+  | encryptedCredential _ _ _ => True
+  | randomNum _ => True
+  | TCG_CSR_IDevID _ _ _ => True
+  | TCG_CSR_LDevID _ _ => True
+  | signedCertificate _ => True
+  | pair _ _ => True
+  | _ => False
   end.
 
 
 
-(* Discoverable relation and Send function are equivalent *)
 
-  Lemma discoverableSend : forall m st,
-    discoverable m st ->
-    send m = st.
-  Proof.
-    intros m st H; induction H; simpl; subst; reflexivity.
-  Qed.
 
-  Lemma sendDiscoverable' : forall m,
-    discoverable m (send m).
-  Proof.
-    intros m; induction m; simpl; constructor; assumption.
-  Qed.
 
-  Lemma sendDiscoverable : forall m st,
-    send m = st -> 
-    discoverable m st.
-  Proof.
-    intros m st H; induction m; subst; apply sendDiscoverable'.
-  Qed.
 
-  Theorem iff_DiscoverableSend : forall m st,
-    discoverable m st <-> send m = st.
+
+
+(* Owner creation of LAK certificate based on IAK certificate *)
+(* **************************************************************** *)
+
+
+(*
+... ;; MakePair csr sig ;; ...
+*)
+Fixpoint isSuperseqOfStep5_Owner (seq : sequence) (csr sig : message) : Prop :=
+  match seq with
+  | c ;; s =>
+      match c with
+      | MakePair m1 m2 =>
+          if (decEq csr m1)
+          then (
+            if (decEq sig m2)
+            then True (* Done *)
+            else isSuperseqOfStep5_Owner s csr sig )
+          else isSuperseqOfStep5_Owner s csr sig
+      | _ => isSuperseqOfStep5_Owner s csr sig
+      end
+  | Done => False
+  end.
+
+Lemma isSuperseqOfStep5_Owner_lemma : forall s iniTPM ini finTPM fin csr sig,
+  seq_execute (iniTPM, ini) s (finTPM, fin) ->
+  In (pair csr sig) fin ->
+  ~ (In (pair csr sig) ini) ->
+  isSuperseqOfStep5_Owner s csr sig.
+Proof.
+  induction s; intros iniTPM ini finTPM fin csr sig E I N0.
+  - destruct c; simpl in *; inversion E; inversion H2; 
+    subst; try (eapply IHs; fdeq);
+    destruct (decEq csr m);
+    destruct (decEq sig m0);
+    subst; trivial;
+    eapply IHs; fdeq.
+  - inversion E; subst; congruence.
+Qed.
+
+
+(*
+... ;; TPM2_Sign hsh (pubToPrivKey lak) ;; 
+... ;; MakePair csr (signature hsh (pubToPrivKey lak)) ;; ...
+*)
+Fixpoint isSuperseqOfSteps4to5_Owner (seq : sequence) (hsh csr : message) (lak : pubKey) : Prop :=
+  match seq with
+  | c ;; s =>
+      match c with
+      | TPM2_Sign m k =>
+          if (decEq hsh m)
+          then (
+            if (decEq (pubToPrivKey lak) k)
+            then isSuperseqOfStep5_Owner s csr (signature hsh (pubToPrivKey lak))  (* Find next *)
+            else isSuperseqOfSteps4to5_Owner s hsh csr lak )
+          else isSuperseqOfSteps4to5_Owner s hsh csr lak
+      | _ => isSuperseqOfSteps4to5_Owner s hsh csr lak
+      end
+  | Done => False
+  end.
+
+Lemma isSuperseqOfSteps4to5_Owner_lemma : forall s iniTPM ini finTPM fin hsh csr lak,
+  seq_execute (iniTPM, ini) s (finTPM, fin) ->
+  In (pair csr (signature hsh (pubToPrivKey lak))) fin ->
+  ~ (In (pair csr (signature hsh (pubToPrivKey lak))) ini) ->
+  ~ (In (signature hsh (pubToPrivKey lak)) ini) ->
+  (forall k, hsh <> TPM2B_Attest k) ->
+  isSuperseqOfSteps4to5_Owner s hsh csr lak.
+Proof.
+  induction s; intros iniTPM ini finTPM fin hsh csr lak E I N0 N1 NA.
+  - destruct c; simpl in *; inversion E; inversion H2; 
+    subst; try (eapply IHs; fdeq);
+    destruct (decEq hsh m);
+    try destruct (decEq (pubToPrivKey lak) (Private i Restricting Signing d f));
+    try destruct (decEq (pubToPrivKey lak) (Private i NonRestricting Signing d f));
+    subst; try eapply IHs; try eapply isSuperseqOfStep5_Owner_lemma; fdeq.
+  - inversion E; subst; congruence.
+Qed.
+
+
+(*
+... ;; TPM2_Hash csr ;;
+... ;; TPM2_Sign (hash csr) (pubToPrivKey lak) ;;
+... ;; MakePair csr (signature (hash csr) (pubToPrivKey lak)) ;; ...
+*)
+Fixpoint isSuperseqOfSteps3to5_Owner (seq : sequence) (csr : message) (lak : pubKey) : Prop :=
+  match seq with
+  | c ;; s => 
+      match c with 
+      | TPM2_Hash m => 
+          if (decEq csr m)
+          then isSuperseqOfSteps4to5_Owner s (hash m) m lak (* Find next *)
+          else isSuperseqOfSteps3to5_Owner s csr lak
+      | _ => isSuperseqOfSteps3to5_Owner s csr lak
+      end
+  | Done => False
+  end.
+
+Lemma isSuperseqOfSteps3to5_Owner_lemma : forall s iniTPM ini finTPM fin csr lak,
+  seq_execute (iniTPM, ini) s (finTPM, fin) ->
+  In (pair csr (signature (hash csr) (pubToPrivKey lak))) fin ->
+  ~ (In (pair csr (signature (hash csr) (pubToPrivKey lak))) ini) ->
+  ~ (In (signature (hash csr) (pubToPrivKey lak)) ini) ->
+  ~ (In (hash csr) ini) ->
+  ~ (In (hash csr) iniTPM) ->
+  isSuperseqOfSteps3to5_Owner s csr lak.
+Proof.
+  induction s; intros iniTPM ini finTPM fin csr lak E I N0 N1 N2 N3.
+  - destruct c; simpl in *; inversion E; inversion H2; 
+    subst; try (eapply IHs; fdeq);
+    destruct (decEq csr m);
+    subst; try eapply IHs; try eapply isSuperseqOfSteps4to5_Owner_lemma; fdeq.
+  - inversion E; subst; congruence.
+Qed.
+
+
+(*
+... ;; MakeCSR_LDevID attest cert ;;
+... ;; TPM2_Hash (TCG_CSR_LDevID attest cert) ;;
+... ;; TPM2_Sign (hash (TCG_CSR_LDevID attest cert)) (pubToPrivKey lak) ;;
+... ;; MakePair (TCG_CSR_LDevID attest cert) 
+                (signature (hash (TCG_CSR_LDevID attest cert)) (pubToPrivKey lak)) ;; ...
+*)
+Fixpoint isSuperseqOfSteps2to5_Owner (seq : sequence) (attest : message) (cert : signedCert) (lak : pubKey) : Prop :=
+  match seq with
+  | c ;; s => 
+      match c with
+      | MakeCSR_LDevID m crt => 
+          if (decEq attest m) 
+          then (
+            if (decEq cert crt)
+            then isSuperseqOfSteps3to5_Owner s (TCG_CSR_LDevID m crt) lak (* Find next *)
+            else isSuperseqOfSteps2to5_Owner s attest cert lak )
+          else isSuperseqOfSteps2to5_Owner s attest cert lak
+      | _ => isSuperseqOfSteps2to5_Owner s attest cert lak
+      end
+  | Done => False
+  end.
+
+Lemma isSuperseqOfSteps2to5_Owner_lemma : forall s iniTPM ini finTPM fin attest cert lak,
+  seq_execute (iniTPM, ini) s (finTPM, fin) ->
+  In (pair (TCG_CSR_LDevID attest cert)
+           (signature (hash (TCG_CSR_LDevID attest cert)) (pubToPrivKey lak))) fin ->
+  ~ (In (pair (TCG_CSR_LDevID attest cert)
+              (signature (hash (TCG_CSR_LDevID attest cert)) (pubToPrivKey lak))) ini) ->
+  ~ (In (signature (hash (TCG_CSR_LDevID attest cert)) (pubToPrivKey lak)) ini) ->
+  ~ (In (hash (TCG_CSR_LDevID attest cert)) ini) ->
+  ~ (In (hash (TCG_CSR_LDevID attest cert)) iniTPM) ->
+  ~ (In (TCG_CSR_LDevID attest cert) ini) ->
+  isSuperseqOfSteps2to5_Owner s attest cert lak.
+Proof.
+  induction s; intros iniTPM ini finTPM fin attest cert lak E I N0 N1 N2 N2_TPM N3.
+  - destruct c; simpl in *; inversion E; inversion H2; 
+    subst; try (eapply IHs; fdeq).
+    destruct (decEq attest m);
+    destruct (decEq cert s0);
+    subst; try eapply IHs; try eapply isSuperseqOfSteps3to5_Owner_lemma; fdeq.
+  - inversion E; subst; congruence.
+Qed.
+
+
+(*
+... ;; TPM2_Certify lak (pubToPrivKey iak) ;;
+... ;; MakeCSR_LDevID (signature (TPM2B_Attest lak) (pubToPrivKey iak)) cert ;;
+... ;; TPM2_Hash 
+          (TCG_CSR_LDevID (signature (TPM2B_Attest lak) (pubToPrivKey iak)) cert) ;;
+... ;; TPM2_Sign 
+          (hash (TCG_CSR_LDevID (signature (TPM2B_Attest lak) (pubToPrivKey iak)) cert)) 
+          (pubToPrivKey lak) ;;
+... ;; MakePair 
+          (TCG_CSR_LDevID (signature (TPM2B_Attest lak) (pubToPrivKey iak)) cert) 
+          (signature 
+            (hash (TCG_CSR_LDevID (signature (TPM2B_Attest lak) (pubToPrivKey iak)) cert)) 
+            (pubToPrivKey lak)) ;; ...
+*)
+Fixpoint isSuperseqOfSteps1to5_Owner (seq : sequence) (iak lak : pubKey) (cert : signedCert) : Prop :=
+  match seq with
+  | c ;; s => 
+      match c with
+      | TPM2_Certify k k0' => 
+          if (decEq lak k)
+          then (
+            if (decEq (pubToPrivKey iak) k0')
+            then isSuperseqOfSteps2to5_Owner s (signature (TPM2B_Attest k) k0') cert k  (* Find next *)
+            else isSuperseqOfSteps1to5_Owner s iak lak cert )
+          else isSuperseqOfSteps1to5_Owner s iak lak cert
+      | _ => isSuperseqOfSteps1to5_Owner s iak lak cert
+      end
+  | Done => False
+  end.
+
+Lemma isSuperseqOfSteps1to5_Owner_lemma : forall s iniTPM ini finTPM fin iak lak cert,
+  seq_execute (iniTPM, ini) s (finTPM, fin) ->
+  In (pair (TCG_CSR_LDevID (signature (TPM2B_Attest lak) (pubToPrivKey iak)) cert)
+           (signature 
+              (hash (TCG_CSR_LDevID (signature (TPM2B_Attest lak) (pubToPrivKey iak)) cert)) 
+              (pubToPrivKey lak))) fin ->
+  ~ (In (pair (TCG_CSR_LDevID (signature (TPM2B_Attest lak) (pubToPrivKey iak)) cert)
+              (signature 
+                  (hash (TCG_CSR_LDevID (signature (TPM2B_Attest lak) (pubToPrivKey iak)) cert)) 
+                  (pubToPrivKey lak))) ini) ->
+  ~ (In (signature 
+          (hash (TCG_CSR_LDevID (signature (TPM2B_Attest lak) (pubToPrivKey iak)) cert)) 
+          (pubToPrivKey lak)) ini) ->
+  ~ (In (hash (TCG_CSR_LDevID (signature (TPM2B_Attest lak) (pubToPrivKey iak)) cert)) ini) ->
+  ~ (In (hash (TCG_CSR_LDevID (signature (TPM2B_Attest lak) (pubToPrivKey iak)) cert)) iniTPM) ->
+  ~ (In (TCG_CSR_LDevID (signature (TPM2B_Attest lak) (pubToPrivKey iak)) cert) ini) ->
+  ~ (In (signature (TPM2B_Attest lak) (pubToPrivKey iak)) ini) ->
+  ~ (In (TPM2B_Attest lak) ini) ->
+  ~ (In (TPM2B_Attest lak) iniTPM) ->
+  isSuperseqOfSteps1to5_Owner s iak lak cert.
+Proof.
+  induction s; intros iniTPM ini finTPM fin iak lak cert E I N0 N1 N2 N2_TPM N3 N4 N5 N5_TPM.
+  - destruct c; simpl in *; inversion E; inversion H2;  
+    subst; try (eapply IHs; fdeq).
+    destruct (decEq lak (Public i r s1 d f));
+    destruct (decEq (pubToPrivKey iak) (Private i0 r0 Signing d0 f0));
+    subst; try eapply IHs; try eapply isSuperseqOfSteps2to5_Owner_lemma; try fdeq;
+    try (rewrite <- e0; assumption).
+  - inversion E; subst; congruence.
+Qed.
+
+
+
+Module Type LAK_Cert_Protocol.
+
+
+(* Owner parameters *)
+  Parameter pubLAK : pubKey.
+  Parameter pubIAK : pubKey.
+  Parameter certIAK : signedCert.
+
+(* CA parameters *)
+  Parameter pubCA : pubKey.
+  Parameter pubOEM : pubKey.
+
+(* All keys must be distinct *)
+  Axiom keys_distinct :
+    pubLAK <> pubIAK /\
+    pubLAK <> pubCA /\
+    pubLAK <> pubOEM /\
+    pubIAK <> pubCA /\
+    pubIAK <> pubOEM /\
+    pubCA <> pubOEM.
+
+  Definition privLAK := pubToPrivKey pubLAK.
+  Definition privIAK := pubToPrivKey pubIAK.
+  Definition privCA := pubToPrivKey pubCA.
+
+
+
+
+
+(* Correct protocol steps of owner *)
+  Definition steps1to5_Owner : sequence :=
+    TPM2_Certify pubLAK privIAK ;;
+    MakeCSR_LDevID (signature (TPM2B_Attest pubLAK) privIAK) certIAK ;;
+    TPM2_Hash (TCG_CSR_LDevID (signature (TPM2B_Attest pubLAK) privIAK) certIAK) ;;
+    TPM2_Sign (hash (TCG_CSR_LDevID (signature (TPM2B_Attest pubLAK) privIAK) certIAK)) privLAK ;;
+    MakePair (TCG_CSR_LDevID (signature (TPM2B_Attest pubLAK) privIAK) certIAK) 
+             (signature (hash (TCG_CSR_LDevID (signature (TPM2B_Attest pubLAK) privIAK) certIAK)) privLAK) ;;
+    Done.
+
+
+
+(* The CA is trusted to have a good initial state *)
+Definition iniTPM_CA : tpm_state :=
+  [ privateKey privCA ;
+    publicKey pubCA ].
+
+  Definition ini_CA : state :=
+  [ publicKey pubOEM ;
+    privateKey privCA ;
+    publicKey pubCA ].
+
+  Axiom CA_keys_good :
+    caKey pubCA /\
+    caKey pubOEM.
+
+(* Protocol steps of CA *)
+(* The CA waits to recieve a message from the owner. *)
+(* That message must be in a specific form to be considered a proper request. *)
+(* The CA will then execute its protocol steps on the input message. *)
+(* If the protocol succeeds the CA will issue certificate [Cert k_LAK id privCA] to the owner. *)
+  Definition steps_CA (msg : message) (iak lak : pubKey) (cert : signedCert) : Prop :=
+    match msg with
+    | (pair (TCG_CSR_LDevID (signature (TPM2B_Attest k) k0') 
+                            (Cert k0 id k_ca'))
+            (signature m k')) =>
+          iak = k0 /\
+          lak = k /\
+          cert = (Cert k0 id k_ca') /\
+          seq_execute (iniTPM_CA, inferFrom msg ++ ini_CA)
+                            (CheckHash m
+                                      (TCG_CSR_LDevID (signature (TPM2B_Attest k) k0') 
+                                                      (Cert k0 id k_ca')) ;;
+                            CheckSig (signature m k') k ;;
+                            CheckSig (signature (TPM2B_Attest k) k0') k0 ;;
+                            CheckCert (Cert k0 id k_ca') pubOEM ;;
+                            CheckAttributes k Restricting Signing NonDecrypting Fixing ;;
+                            Done)
+                            (iniTPM_CA, 
+                            inferFrom msg ++ ini_CA)
+    | _ => False
+    end.
+
+
+
+
+
+(* Minimal initial state pair of owner *)
+
+  Definition iniTPM_Owner : tpm_state :=
+  [ privateKey privLAK ;
+    privateKey privIAK ].
+
+  Definition ini_Owner : state :=
+  [ signedCertificate certIAK ].
+
+
+
+(* Minimality proof part 1 *)
+  Lemma ini_Owner_lowerBound : forall iniTPM ini fin,
+    seq_execute (iniTPM, ini) steps1to5_Owner fin ->
+    (iniTPM_Owner \subsetOf iniTPM) /\
+    (ini_Owner \subsetOf ini).
   Proof.
+    intros iniTPM ini fin E;
+(* Split steps_Owner into its individual commands *)
+    inversion E as [initial mid1 final command steps_Owner' H_Certify E1| ]; subst;
+    inversion E1 as [initial mid2 final command steps_Owner' H_MakeCSR E2| ]; subst;
+    inversion E2 as [initial mid3 final command steps_Owner' H_Hash E3| ]; subst;
+    inversion E3 as [initial mid4 final command steps_Owner' H_Sign E4| ]; subst;
+    inversion E4 as [initial mid5 final command steps_Owner' H_MakePair E5| ]; subst;
+    inversion E5; subst;
+(* Invert each individual step in reverse order *) 
+    inversion H_MakePair; subst; 
+    inversion H_Sign; subst;
+    inversion H_Hash; subst;
+    inversion H_MakeCSR; subst;
+    inversion H_Certify; subst;
+(* Clear all hypothesis other than state requirements and key definitions *)
+    clear E E1 E2 E3 E4 E5;
+    clear H_Certify H_MakeCSR H_Hash H_Sign H_MakePair;
     split.
-    - apply discoverableSend.
-    - apply sendDiscoverable.
+(* Case TPM state with Restricted Signing key *)
+    - unfold iniTPM_Owner; intros m I; inversion I; subst.
+    -- rewrite <- H0; inversion H5 as [EQ_false | H5']; subst.
+        inversion EQ_false.
+        assumption.
+    -- inversion H; subst.
+    --- rewrite <- H10; assumption.
+    --- inversion H1.
+(* Case state with Restricted Signing key *)
+    - unfold ini_Owner; intros m I; inversion I; subst.
+    -- inversion H11 as [EQ_false | H11']; subst.
+        inversion EQ_false.
+        assumption.
+    -- inversion H.
+(* Case TPM state with Non-Restricted Signing key *)
+    - unfold iniTPM_Owner; intros m I; inversion I; subst.
+    -- rewrite <- H0; inversion H5 as [EQ_false | H5']; subst. 
+        inversion EQ_false.
+        assumption.
+    -- inversion H; subst.
+    --- rewrite <- H10; assumption.
+    --- inversion H1.
+(* Case state with Non-Restricted Signing key *)
+    - unfold ini_Owner; intros m I; inversion I; subst.
+    -- inversion H11 as [EQ_false | H11']; subst. 
+         inversion EQ_false.
+         assumption.
+    -- inversion H.
   Qed.
 
 
 
 
 
+(* Minimality proof part 2 *)
+  Lemma ini_Owner_sufficient : forall msg,
+    attestationKey pubIAK ->
+    steps_CA msg pubIAK pubLAK certIAK ->
+    exists fin, seq_execute (iniTPM_Owner, ini_Owner) steps1to5_Owner fin.
+  Proof. 
+    intros m goodIAK CA;
+    unfold iniTPM_Owner, ini_Owner, steps1to5_Owner, privIAK, privLAK;
+    destruct pubIAK, r, s, d, f; simpl in goodIAK; try inversion goodIAK;
+    destruct m; try inversion CA;
+    destruct m1; try inversion CA;
+    destruct m1; try inversion CA;
+    destruct m1; try inversion CA;
+    destruct s; try inversion CA;
+    destruct m2; try inversion CA; subst;
+    destruct H0; subst; destruct H0; subst;
+    clear CA; simpl in *;
+    inversion H0 as [initial mid1 final command steps_Owner' H_CheckHash H1 | ]; subst; 
+    inversion H1 as [initial mid2 final command steps_Owner' H_CheckSig1 H2 | ]; subst;
+    inversion H2 as [initial mid3 final command steps_Owner' H_CheckSig2 H3 | ]; subst;
+    inversion H3 as [initial mid4 final command steps_Owner' H_CheckCert H4 | ]; subst;
+    inversion H4 as [initial mid5 final command steps_Owner' H_CheckAttributes H5 | ]; subst;
+    inversion H5; subst;
+    inversion H_CheckAttributes; subst;
+    simpl; trivial;
+    eexists; simpl; repeat eapply SE_Seq; econstructor; simpl; auto.
+  Qed.
 
 
+  Axiom correct_Owner : forall finTPM fin,
+    seq_execute (iniTPM_Owner, ini_Owner) steps1to5_Owner (finTPM, fin) ->
+    exists msg, In msg fin /\ steps_CA msg pubIAK pubLAK certIAK.
+
+
+
+  Lemma ca_implies_isSuperseqOfSteps1to5 : forall s iniTPM ini finTPM fin msg iak lak cert,
+    seq_execute (iniTPM, ini) s (finTPM, fin) ->
+    In msg fin ->
+    (forall m', needsGeneratedTPM m' -> ~ In m' iniTPM) ->
+    (forall m', needsGenerated m' -> ~ In m' ini) ->
+    steps_CA msg iak lak cert -> 
+    isSuperseqOfSteps1to5_Owner s iak lak cert.
+  Proof.
+    intros s iniTPM ini finTPM fin m iak lak cert E I N_TPM N CA.
+(* Get m into the form of the match statement in steps_CA *)
+    destruct m; try inversion CA;
+    destruct m1; try inversion CA;
+    destruct m1; try inversion CA;
+    destruct m1; try inversion CA;
+    destruct s0; try inversion CA;
+    destruct m2; try inversion CA; subst;
+    destruct H0; subst; destruct H0; subst;
+    clear CA; simpl in *.
+(* Split steps_CA into its individual commands *)
+    inversion H0 as [initial mid1 final command steps_Owner' H_CheckHash H1 | ]; subst; 
+    inversion H1 as [initial mid2 final command steps_Owner' H_CheckSig1 H2 | ]; subst;
+    inversion H2 as [initial mid3 final command steps_Owner' H_CheckSig2 H3 | ]; subst;
+    inversion H3 as [initial mid4 final command steps_Owner' H_CheckCert H4 | ]; subst;
+    inversion H4 as [initial mid5 final command steps_Owner' H_CheckAttributes H5 | ]; subst;
+    inversion H5; subst;
+(* Invert each individual step in reverse order *) 
+    inversion H_CheckAttributes; subst;
+    inversion H_CheckCert; subst;
+    inversion H_CheckSig2; subst;
+    inversion H_CheckSig1; subst;
+    inversion H_CheckHash; subst.
+(* Apply lemma *)
+    eapply isSuperseqOfSteps1to5_Owner_lemma; eauto; 
+    try apply N; try apply N_TPM; simpl; trivial.
+  Qed.
+
+
+
+  Lemma isSuperseqOfSteps1to5_implies_certify : forall s iak lak cert,
+    isSuperseqOfSteps1to5_Owner s iak lak cert ->
+    command_in_sequence (TPM2_Certify lak (pubToPrivKey iak)) s.
+  Proof.
+    induction s; intros iak lak cert H0.
+    - simpl; destruct (decEq (TPM2_Certify lak (pubToPrivKey iak)) c);
+      [ trivial
+      | apply IHs with (cert := cert);
+        destruct c; simpl in *; try fdeq ].
+      destruct (decEq lak p); 
+      destruct (decEq (pubToPrivKey iak) p0); subst; congruence.
+    - inversion H0.
+  Qed.
+(*
+  Lemma isSuperseqOfSteps1to5_Owner_implies_sign : forall s iak lak cert,
+    isSuperseqOfSteps1to5_Owner s iak lak cert ->
+    exists hsh, command_in_sequence s (TPM2_Sign hsh (pubToPrivKey lak)).
+  Proof.
+    intros s iak lak cert H0.
+    exists (hash (TCG_CSR_LDevID (signature (TPM2B_Attest pubLAK) privIAK) certIAK)).
+    generalize dependent cert. generalize dependent lak. generalize dependent iak.
+    induction s; intros.
+    simpl. destruct (decEq
+    (TPM2_Sign
+       (hash
+          (TCG_CSR_LDevID
+             (signature (TPM2B_Attest pubLAK) privIAK) certIAK))
+       (pubToPrivKey lak)) c).
+       trivial.
+      eapply IHs. destruct c; try (simpl in *; fdeq; fail). simpl in *.
+      destruct (decEq lak p);
+      destruct (decEq (pubToPrivKey iak) p0); subst; try congruence.
+*)
+  Lemma certify_implies_lakInTPM : forall s iniTPM ini finTPM fin iak lak,
+    seq_execute (iniTPM, ini) s (finTPM, fin) -> 
+    command_in_sequence (TPM2_Certify lak (pubToPrivKey iak)) s ->
+    In (privateKey (pubToPrivKey lak)) iniTPM.
+  Proof.
+    induction s; intros iniTPM ini finTPM fin iak lak E CI.
+    - simpl in *; destruct (decEq (TPM2_Certify lak (pubToPrivKey iak)) c); inversion E; subst.
+    -- inversion H2; assumption.
+    -- destruct mid as [midTPM mid]; eapply exec_cannotGenerateKey; eauto.
+    - inversion CI.
+  Qed.
+
+
+  Lemma certify_implies_iakInTPM : forall s iniTPM ini finTPM fin iak lak,
+    seq_execute (iniTPM, ini) s (finTPM, fin) -> 
+    command_in_sequence (TPM2_Certify lak (pubToPrivKey iak)) s ->
+    In (privateKey (pubToPrivKey iak)) iniTPM.
+  Proof.
+    induction s; intros iniTPM ini finTPM fin iak lak E CI.
+    - simpl in *; destruct (decEq (TPM2_Certify lak (pubToPrivKey iak)) c); inversion E; subst.
+    -- inversion H2; assumption.
+    -- destruct mid as [midTPM mid]; eapply exec_cannotGenerateKey; eauto.
+    - inversion CI.
+  Qed.
+
+
+
+
+(* PROTOCOL ASSURANCES *)
+
+(* Given the following assumptions: 
+      The Owner executes some sequence of steps
+      resulting in a message in its final state
+      when only keys and certificates may be in its initial states.
+      The CA's protocol executes successfully on the given message.
+  Conclude:
+      The private IAK and private LAK reside in the same TPM *)
+  Theorem lak_and_iak_in_TPM : forall s iniTPM ini finTPM fin msg iak lak cert,
+    seq_execute (iniTPM, ini) s (finTPM, fin) -> 
+    In msg fin ->
+    (forall m', needsGeneratedTPM m' -> ~ In m' iniTPM) ->
+    (forall m', needsGenerated m' -> ~ In m' ini) ->
+    steps_CA msg iak lak cert ->
+    In (privateKey (pubToPrivKey lak)) iniTPM /\ In (privateKey (pubToPrivKey iak)) iniTPM.
+  Proof.
+    intros s iniTPM ini finTPM fin m iak lak cert E I N_TPM N CA; 
+    split; [ eapply certify_implies_lakInTPM | eapply certify_implies_iakInTPM ];
+    eauto; eapply isSuperseqOfSteps1to5_implies_certify; eapply ca_implies_isSuperseqOfSteps1to5; eauto.
+  Qed.
+
+(* Conclude:
+      The LAK is a Restricted Signing NonDecrypting key *)
+    Theorem lak_good_attributes : forall msg iak lak cert,
+      steps_CA msg iak lak cert ->
+      attestationKey lak.
+    Proof.
+      intros m iak lak cert CA;
+      destruct m; try inversion CA;
+      destruct m1; try inversion CA;
+      destruct m1; try inversion CA;
+      destruct m1; try inversion CA;
+      destruct s; try inversion CA;
+      destruct m2; try inversion CA; subst;
+      destruct H0; subst; destruct H0; subst;
+      clear CA; simpl in *.
+      inversion H0 as [initial mid1 final command steps_Owner' H_CheckHash H1 | ]; subst; 
+      inversion H1 as [initial mid2 final command steps_Owner' H_CheckSig1 H2 | ]; subst;
+      inversion H2 as [initial mid3 final command steps_Owner' H_CheckSig2 H3 | ]; subst;
+      inversion H3 as [initial mid4 final command steps_Owner' H_CheckCert H4 | ]; subst;
+      inversion H4 as [initial mid5 final command steps_Owner' H_CheckAttributes H5 | ]; subst;
+      inversion H5; subst;
+      inversion H_CheckAttributes; subst;
+      simpl; trivial.
+    Qed.
+
+
+  
+
+
+(*
+  Theorem control_of_lak : forall s iniTPM ini finTPM fin m iak lak cert,
+    seq_execute (iniTPM, ini) s (finTPM, fin) -> 
+    In m fin ->
+    (forall m', needsGenerated m' -> ~ In m' iniTPM) ->
+    (forall m', needsGenerated m' -> ~ In m' ini) ->
+    steps_CA m iak lak cert ->
+    exists hsh, command_in_sequence s (TPM2_Sign hsh (pubToPrivKey lak)).
+*)
+
+End LAK_Cert_Protocol.
+
+
+
+
+
+(*
+Module goodLAK <: LAK_Cert_Protocol.
+
+(* Owner parameters *)
+  Definition pubNewKey : pubKey := Public 52 Restricting Signing NonDecrypting.
+  Definition pubIAK : pubKey := Public 51 Restricting Signing NonDecrypting.
+  Definition certIAK : signedCert := Cert (Public 51 Restricting Signing NonDecrypting) (Device_info 5) (Private 1 NonRestricting Signing NonDecrypting).
+
+(* CA parameters *)
+  Definition pubCA : pubKey := Public 2 NonRestricting Signing NonDecrypting.
+  Definition privCA : privKey := Private 2 NonRestricting Signing NonDecrypting.
+  Definition pubOEM : pubKey := Public 1 NonRestricting Signing NonDecrypting.
+
+
+  Theorem keys_distinct :
+    pubNewKey <> pubIAK /\
+    pubNewKey <> pubCA /\
+    pubNewKey <> pubOEM /\
+    pubIAK <> pubCA /\
+    pubIAK <> pubOEM /\
+    pubCA <> pubOEM.
+  Proof.
+    repeat split; intros contra; inversion contra.
+  Qed.
+
+
+  Definition privLAK := pubToPrivKey pubNewKey.
+  Definition privIAK := pubToPrivKey pubIAK.
+
+
+  Definition iniTPM_Owner : tpm_state :=
+  [ privateKey privLAK ;
+    privateKey privIAK ].
+
+  Definition ini_Owner : state :=
+  [ publicKey pubNewKey ;
+    signedCertificate certIAK ].
+
+
+  Definition steps_Owner : sequence :=
+  TPM2_Certify pubNewKey privIAK ;;
+  MakeCSR_LDevID (signature (TPM2B_Attest pubNewKey) privIAK) certIAK ;;
+  TPM2_Hash (TCG_CSR_LDevID (signature (TPM2B_Attest pubNewKey) privIAK) certIAK) ;;
+  TPM2_Sign (hash (TCG_CSR_LDevID (signature (TPM2B_Attest pubNewKey) privIAK) certIAK)) privLAK ;;
+  MakePair (TCG_CSR_LDevID (signature (TPM2B_Attest pubNewKey) privIAK) certIAK) 
+           (signature (hash (TCG_CSR_LDevID (signature (TPM2B_Attest pubNewKey) privIAK) certIAK)) privIAK) ;;
+  Done.
+
+
+
+
+  Theorem steps_lowerBound : forall iniTPM ini fin,
+    seq_execute (iniTPM, ini) steps_Owner fin ->
+    (iniTPM_Owner \subsetOf iniTPM) /\
+    (ini_Owner \subsetOf ini).
+  Proof.
+    intros iniTPM ini fin E.
+
+    inversion E as [initial mid1 final command steps_Owner' E_Certify E'| ]; subst. 
+    inversion E' as [initial mid2 final command steps_Owner' E_MakeCSR E''| ]; subst.
+    inversion E'' as [initial mid3 final command steps_Owner' E_Hash E'''| ]; subst.
+    inversion E''' as [initial mid4 final command steps_Owner' E_Sign E''''| ]; subst.
+    inversion E'''' as [initial mid5 final command steps_Owner' E_MakePair E'''''| ]; subst.
+    inversion E'''''; subst.
+
+    inversion E_MakePair; subst; 
+    inversion E_Sign; subst;
+    inversion E_Hash; subst;
+    inversion E_MakeCSR; subst;
+    inversion E_Certify; subst;
+
+    clear E E' E'' E''' E'''' E''''';
+    clear E_Certify E_MakeCSR E_Hash E_Sign E_MakePair;
+    split.
+
+    - unfold iniTPM_Owner; intros m I; inversion I; subst.
+    -- unfold privIAK; simpl; inversion H3 as [EQ_false | H3']; subst.
+        inversion EQ_false.
+       inversion H3' as [EQ_false | H3'']; subst. 
+        inversion EQ_false.
+        assumption.
+    -- inversion H; subst.
+    --- unfold privIAK; simpl. assumption.
+    --- inversion H0.
+
+    - unfold ini_Owner; intros m I; inversion I; subst.
+    -- unfold pubNewKey; simpl; assumption.
+    -- inversion H; subst.
+    --- inversion H10 as [EQ_false | H10']; subst. 
+         inversion EQ_false.
+         assumption.
+    --- inversion H0.
+Qed.
+
+
+
+
+  Theorem steps_min : exists fin,
+    seq_execute (iniTPM_Owner, ini_Owner) steps_Owner fin.
+  Proof.
+    eexists; unfold iniTPM_Owner; unfold ini_Owner; unfold steps_Owner;
+    unfold privIAK; unfold privIAK; unfold certIAK;
+    unfold pubNewKey; unfold pubIAK.
+    repeat eapply E_Seq; constructor; simpl; auto.
+  Qed.
+
+
+
+
+  Definition iniTPM_CA : tpm_state :=
+  [ privateKey privCA ;
+    publicKey pubCA ].
+
+  Definition ini_CA : state :=
+  [ publicKey pubOEM ;
+    privateKey privCA ;
+    publicKey pubCA ].
+
+  Theorem CA_keys_good :
+    privCA = pubToPrivKey pubCA /\
+    caKey pubCA /\
+    caKey pubOEM.
+  Proof. 
+    repeat split.
+  Qed.
+
+
+
+  Definition steps_CA (m : message) : Prop :=
+    match m with
+    | ((TCG_CSR_LDevID (signature (TPM2B_Attest k) k_IAK') 
+                       (Cert k_IAK id k_OEM')),,
+       (signature m k')) =>
+          seq_execute (iniTPM_CA, inferFrom m ++ ini_CA)
+                           (CheckHash m 
+                                     (TCG_CSR_LDevID (signature (TPM2B_Attest k) k_IAK') 
+                                                     (Cert k_IAK id k_OEM')) ;;
+                            CheckSig (signature m k') k ;;
+                            CheckSig (signature (TPM2B_Attest k) k_IAK') k_IAK ;;
+                            CheckCert (Cert k_IAK id k_OEM') pubOEM ;;
+                            CheckAttributes k Restricting Signing NonDecrypting ;;
+                            Done)
+                           (iniTPM_CA, 
+                            inferFrom m ++ ini_CA)
+    | _ => False
+    end.
+
+
+  Theorem correct_Owner : forall finTPM fin,
+    seq_execute (iniTPM_Owner, ini_Owner) steps_Owner (finTPM, fin) ->
+    exists m, In m fin /\ steps_CA m.
+  Proof.
+    intros finTPM fin E. 
+    exists ((TCG_CSR_LDevID (signature (TPM2B_Attest pubNewKey) privIAK) certIAK) ,,
+            (signature (hash (TCG_CSR_LDevID (signature (TPM2B_Attest pubNewKey) privIAK) certIAK)) privIAK)).
+    split.
+    - inversion E as [initial mid1 final command steps_Owner' E_Certify E'| ]; subst. 
+      inversion E' as [initial mid2 final command steps_Owner' E_MakeCSR E''| ]; subst.
+      inversion E'' as [initial mid3 final command steps_Owner' E_Hash E'''| ]; subst.
+      inversion E''' as [initial mid4 final command steps_Owner' E_Sign E''''| ]; subst.
+      inversion E'''' as [initial mid5 final command steps_Owner' E_MakePair E'''''| ]; subst.
+      inversion E'''''; subst.
+      inversion E_MakePair; subst; 
+      inversion E_Sign; subst;
+      inversion E_Hash; subst;
+      inversion E_MakeCSR; subst;
+      inversion E_Certify; subst;
+      clear.
+      simpl; auto.
+    - unfold iniTPM_Owner; unfold ini_Owner; unfold steps_Owner;
+      unfold privIAK; unfold privIAK; unfold certIAK;
+      unfold pubNewKey; unfold pubIAK. simpl.
+      repeat eapply E_Seq; constructor; simpl; auto 11.
+  Qed.
+
+
+End goodLAK.
+*)
 
 
 
@@ -595,70 +1685,253 @@
 (* OEM creation of IAK certificate based on EK certificate *)
 (* ******************************************************* *)
 
-(* Numerical comment tags correspond to respective steps in latex documentation *)
+
+
+(*
+... ;; MakePair csr sig ;; ...
+*)
+Fixpoint isSuperseqOfStep4_OEM (seq : sequence) (csr sig : message) : Prop :=
+  match seq with
+  | c ;; s =>
+      match c with
+      | MakePair m1 m2 =>
+          if (decEq csr m1)
+          then (
+            if (decEq sig m2)
+            then True (* Done *)
+            else isSuperseqOfStep4_OEM s csr sig )
+          else isSuperseqOfStep4_OEM s csr sig
+      | _ => isSuperseqOfStep4_OEM s csr sig
+      end
+  | Done => False
+  end.
+
+Lemma isSuperseqOfStep4_OEM_lemma : forall s iniTPM ini finTPM fin csr sig,
+  seq_execute (iniTPM, ini) s (finTPM, fin) ->
+  In (pair csr sig) fin ->
+  ~ (In (pair csr sig) ini) ->
+  isSuperseqOfStep4_OEM s csr sig.
+Proof.
+  induction s; intros iniTPM ini finTPM fin csr sig E I N0.
+  - destruct c; simpl in *; inversion E; inversion H2; 
+    subst; try (eapply IHs; fdeq);
+    destruct (decEq csr m);
+    destruct (decEq sig m0);
+    subst; trivial; eapply IHs; fdeq.
+  - inversion E; subst; congruence.
+Qed.
+
+
+(*
+... ;; TPM2_Sign hsh (pubToPrivKey iak) ;; 
+... ;; MakePair csr (signature hsh (pubToPrivKey iak)) ;; ...
+*)
+Fixpoint isSuperseqOfSteps3to4_OEM (seq : sequence) (hsh csr : message) (iak : pubKey) : Prop :=
+  match seq with
+  | c ;; s =>
+      match c with
+      | TPM2_Sign m k =>
+          if (decEq hsh m)
+          then (
+            if (decEq (pubToPrivKey iak) k)
+            then isSuperseqOfStep4_OEM s csr (signature hsh (pubToPrivKey iak))  (* Find next *)
+            else isSuperseqOfSteps3to4_OEM s hsh csr iak )
+          else isSuperseqOfSteps3to4_OEM s hsh csr iak
+      | _ => isSuperseqOfSteps3to4_OEM s hsh csr iak
+      end
+  | Done => False
+  end.
+
+Lemma isSuperseqOfSteps3to4_OEM_lemma : forall s iniTPM ini finTPM fin hsh csr iak,
+  seq_execute (iniTPM, ini) s (finTPM, fin) ->
+  In (pair csr (signature hsh (pubToPrivKey iak))) fin ->
+  ~ (In (pair csr (signature hsh (pubToPrivKey iak))) ini) ->
+  ~ (In (signature hsh (pubToPrivKey iak)) ini) ->
+  (forall k, hsh <> TPM2B_Attest k) ->
+  isSuperseqOfSteps3to4_OEM s hsh csr iak.
+Proof.
+  induction s; intros iniTPM ini finTPM fin hsh csr iak E I N0 N1 NA.
+  - destruct c; simpl in *; inversion E; inversion H2; 
+    subst; try (eapply IHs; fdeq);
+    destruct (decEq hsh m);
+    try destruct (decEq (pubToPrivKey iak) (Private i Restricting Signing d f));
+    try destruct (decEq (pubToPrivKey iak) (Private i NonRestricting Signing d f));
+    subst; try eapply IHs; try eapply isSuperseqOfStep5_Owner_lemma; fdeq.
+  - inversion E; subst; congruence.
+Qed.
+
+
+(*
+... ;; TPM2_Hash csr ;;
+... ;; TPM2_Sign (hash csr) (pubToPrivKey iak) ;;
+... ;; MakePair csr (signature (hash csr) (pubToPrivKey iak)) ;; ...
+*)
+Fixpoint isSuperseqOfSteps2to4_OEM (seq : sequence) (csr : message) (iak : pubKey) : Prop :=
+  match seq with
+  | c ;; s => 
+      match c with 
+      | TPM2_Hash m => 
+          if (decEq csr m)
+          then isSuperseqOfSteps3to4_OEM s (hash m) m iak (* Find next *)
+          else isSuperseqOfSteps2to4_OEM s csr iak
+      | _ => isSuperseqOfSteps2to4_OEM s csr iak
+      end
+  | Done => False
+  end.
+
+Lemma isSuperseqOfSteps2to4_OEM_lemma : forall s iniTPM ini finTPM fin csr iak,
+  seq_execute (iniTPM, ini) s (finTPM, fin) ->
+  In (pair csr (signature (hash csr) (pubToPrivKey iak))) fin ->
+  ~ (In (pair csr (signature (hash csr) (pubToPrivKey iak))) ini) ->
+  ~ (In (signature (hash csr) (pubToPrivKey iak)) ini) ->
+  ~ (In (hash csr) ini) ->
+  ~ (In (hash csr) iniTPM) ->
+  isSuperseqOfSteps2to4_OEM s csr iak.
+Proof.
+  induction s; intros iniTPM ini finTPM fin csr iak E I N0 N1 N2 N3.
+  - destruct c; simpl in *; inversion E; inversion H2; 
+    subst; try (eapply IHs; fdeq);
+    destruct (decEq csr m);
+    subst; try eapply IHs; try eapply isSuperseqOfSteps4to5_Owner_lemma; fdeq.
+  - inversion E; subst; congruence.
+Qed.
+
+
+(*
+... ;; MakeCSR_IDevID ident cert iak ;;
+... ;; TPM2_Hash (TCG_CSR_IDevID ident cert iak) ;;
+... ;; TPM2_Sign (hash (TCG_CSR_IDevID ident cert iak)) (pubToPrivKey iak) ;;
+... ;; MakePair (TCG_CSR_IDevID ident cert iak) 
+                (signature (hash (TCG_CSR_IDevID ident cert iak)) (pubToPrivKey iak)) ;; ...
+*)
+Fixpoint isSuperseqOfSteps1to4_OEM (seq : sequence) (ident : identifier) (cert : signedCert) (iak : pubKey) : Prop :=
+  match seq with
+  | c ;; s => 
+      match c with
+      | MakeCSR_IDevID id crt k => 
+          if (decEq ident id)
+          then (
+            if (decEq cert crt)
+            then (
+              if (decEq iak k)
+              then isSuperseqOfSteps2to4_OEM s (TCG_CSR_IDevID id crt k) iak
+              else isSuperseqOfSteps1to4_OEM s ident cert iak )
+            else isSuperseqOfSteps1to4_OEM s ident cert iak )
+          else isSuperseqOfSteps1to4_OEM s ident cert iak 
+      | _ => isSuperseqOfSteps1to4_OEM s ident cert iak 
+      end
+  | Done => False
+  end.
+
+Lemma isSuperseqOfSteps1to4_OEM_lemma : forall s iniTPM ini finTPM fin ident cert iak,
+  seq_execute (iniTPM, ini) s (finTPM, fin) ->
+  In (pair (TCG_CSR_IDevID ident cert iak)
+           (signature (hash (TCG_CSR_IDevID ident cert iak)) (pubToPrivKey iak))) fin ->
+  ~ (In (pair (TCG_CSR_IDevID ident cert iak) 
+              (signature (hash (TCG_CSR_IDevID ident cert iak)) (pubToPrivKey iak))) ini) ->
+  ~ (In (signature (hash (TCG_CSR_IDevID ident cert iak)) (pubToPrivKey iak)) ini) ->
+  ~ (In (hash (TCG_CSR_IDevID ident cert iak)) ini) ->
+  ~ (In (hash (TCG_CSR_IDevID ident cert iak)) iniTPM) ->
+  ~ (In (TCG_CSR_IDevID ident cert iak) ini) ->
+  isSuperseqOfSteps1to4_OEM s ident cert iak.
+Proof.
+  induction s; intros iniTPM ini finTPM fin ident cert iak E I N0 N1 N2 N2_TPM N3.
+  - destruct c; simpl in *; inversion E; inversion H2; 
+    subst; try (eapply IHs; fdeq).
+    destruct (decEq ident i);
+    destruct (decEq cert s0);
+    destruct (decEq iak p);
+    subst; try eapply IHs; try eapply isSuperseqOfSteps2to4_OEM_lemma; fdeq.
+  - inversion E; subst; congruence.
+Qed.
+
+
+
+Fixpoint isSuperseqOfStep7_OEM (seq : sequence) (ek iak : pubKey) (rand : randType) :=
+  match seq with
+  | c ;; s =>
+      match c with
+      | TPM2_ActivateCredential crd k' k0' =>
+          match crd with
+          | encryptedCredential n g k =>
+              match n with
+              | hash m =>
+                  match m with
+                  | publicKey k0 =>
+                      if (decEq rand g)
+                      then (
+                        if (decEq ek k)
+                        then (
+                          if (decEq iak k0)
+                          then (
+                            if (decEq (pubToPrivKey ek) k')
+                            then (
+                              if (decEq (pubToPrivKey iak) k0')
+                              then True
+                              else isSuperseqOfStep7_OEM s ek iak rand )
+                            else isSuperseqOfStep7_OEM s ek iak rand )
+                          else isSuperseqOfStep7_OEM s ek iak rand )
+                        else isSuperseqOfStep7_OEM s ek iak rand )
+                      else isSuperseqOfStep7_OEM s ek iak rand 
+                  | _ => isSuperseqOfStep7_OEM s ek iak rand
+                  end
+              | _ => isSuperseqOfStep7_OEM s ek iak rand
+              end
+          | _ => isSuperseqOfStep7_OEM s ek iak rand
+          end
+      | _ => isSuperseqOfStep7_OEM s ek iak rand
+      end
+  | Done => False
+  end.
+
+
+
+
+
+
 
 Module Type IAK_Cert_Protocol.
 
+
 (* OEM parameters *)
-  Parameter pubNewKey : pubKey.
-  Parameter privNewKey : privKey.
+  Parameter pubIAK : pubKey.
   Parameter pubEK : pubKey.
-  Parameter privEK : privKey.
-  Parameter certEK : message.
+  Parameter certEK : signedCert.
+  Parameter devInfo : deviceInfoType.
 
 (* CA parameters *)
   Parameter pubCA : pubKey.
-  Parameter privCA : privKey.
   Parameter pubTM : pubKey.
-  Parameter r : randType.
-
+  Parameter nonce : randType.
 
 (* All keys must be distinct *)
-  Axiom DistinctKeys :
-    pubNewKey <> pubEK /\
-    pubNewKey <> pubCA /\
-    pubNewKey <> pubTM /\
+  Axiom keys_distinct :
+    pubIAK <> pubEK /\
+    pubIAK <> pubCA /\
+    pubIAK <> pubTM /\
     pubEK <> pubCA /\
     pubEK <> pubTM /\
     pubCA <> pubTM.
 
-
-  Definition iniTPM : tpm_state :=
-  [ publicKey pubNewKey ;
-    privateKey privNewKey ;
-    publicKey pubEK ;
-    privateKey privEK ].
-
-  Definition ini : state :=
-  [ publicKey pubNewKey ;
-    privateKey privNewKey ;
-    certEK ;    (* EK certificate *)
-    publicKey pubEK ;
-    privateKey privEK ].
+  Definition privIAK := pubToPrivKey pubIAK.
+  Definition privEK := pubToPrivKey pubEK.
+  Definition privCA := pubToPrivKey pubCA.
 
 
-  Definition c1 : command :=
-  MakeCSR_IDevID certEK pubNewKey ;;                              (* 1 *)
-  TPM2_Hash (TCG_CSR_IDevID certEK pubNewKey) ;;                  (* 2 *)
-  TPM2_Sign (hash (TCG_CSR_IDevID certEK pubNewKey)) privNewKey.  (* 3 *)
+
+(* Correct protocol first steps of OEM *)
+  Definition steps1to4_OEM : sequence :=
+    MakeCSR_IDevID (Device_info devInfo) certEK pubIAK ;;
+    TPM2_Hash (TCG_CSR_IDevID (Device_info devInfo) certEK pubIAK) ;;
+    TPM2_Sign (hash (TCG_CSR_IDevID (Device_info devInfo) certEK pubIAK)) privIAK ;;
+    MakePair (TCG_CSR_IDevID (Device_info devInfo) certEK pubIAK)
+             (signature (hash (TCG_CSR_IDevID (Device_info devInfo) certEK pubIAK)) privIAK) ;;
+    Done.
 
 
-  Definition midTPM : state :=
-  sign (hash (TCG_CSR_IDevID certEK pubNewKey)) privNewKey ::
-  hash (TCG_CSR_IDevID certEK pubNewKey) ::
-  iniTPM.
-
-  Definition mid : state :=
-  sign (hash (TCG_CSR_IDevID certEK pubNewKey)) privNewKey ::
-  hash (TCG_CSR_IDevID certEK pubNewKey) ::
-  (TCG_CSR_IDevID certEK pubNewKey) ::
-  ini.
-
-(*
-  send ((TCG_CSR_IDevID certEK pubNewKey),, (sign (hash (TCG_CSR_IDevID certEK pubNewKey)) privNewKey))   (* 4 *)
-*)
 
 
+(* The CA is trusted to know have a good initial state *)
   Definition iniTPM_CA : tpm_state :=
   [ privateKey privCA ;
     publicKey pubCA ].
@@ -668,203 +1941,477 @@ Module Type IAK_Cert_Protocol.
     privateKey privCA ;
     publicKey pubCA ].
 
+  Axiom CA_keys_good :
+    caKey pubCA /\
+    caKey pubTM.
 
-  Definition c1_CA : command :=
-  CheckHash (hash (TCG_CSR_IDevID certEK pubNewKey)) (TCG_CSR_IDevID certEK pubNewKey) ;; (* 5a *)
-  CheckSig (sign (hash (TCG_CSR_IDevID certEK pubNewKey)) privNewKey) pubNewKey ;;        (* 5b *)
-  CheckCert certEK pubTM ;;                                                               (* 5c *)
-  CheckAttributes pubNewKey Restricted Signing NonDecrypting ;;                           (* 5d *)
-  TPM2_Hash (publicKey pubNewKey) ;;                                                      (* 6 *)
-  TPM2_GetRandom r ;;                                                                     (* 7 *)
-  TPM2_MakeCredential (hash (publicKey pubNewKey)) r pubEK.                               (* 8 *)
-
-
-  Definition midTPM_CA : tpm_state :=
-  encrypt (credential (hash (publicKey pubNewKey)) r) pubEK ::
-  rand r ::
-  hash (publicKey pubNewKey) ::
-  iniTPM_CA.
-
-  Definition mid_CA : state :=
-  encrypt (credential (hash (publicKey pubNewKey)) r) pubEK ::
-  rand r ::
-  hash (publicKey pubNewKey) ::
-  send ((TCG_CSR_IDevID certEK pubNewKey),, (sign (hash (TCG_CSR_IDevID certEK pubNewKey)) privNewKey)) ++
-  ini_CA.
-
-(*
-  send (encrypt (credential (hash (publicKey pubNewKey)) r) pubEK)    (* 9 *)
-*)
-
-  Definition c2 : command :=
-  TPM2_ActivateCredential (encrypt (credential (hash (publicKey pubNewKey)) r) pubEK) privEK (privNewKey).  (* 10 *)
-
-
-  Definition finTPM : tpm_state :=
-  rand r ::
-  credential (hash (publicKey pubNewKey)) r ::
-  midTPM.
-
-  Definition fin : state :=
-  rand r ::
-  credential (hash (publicKey pubNewKey)) r  ::
-  send (encrypt (credential (hash (publicKey pubNewKey)) r) pubEK) ++
-  mid.
-
-(*
-  send (rand r)    (* 11 *)
-*)
-
-  Definition c2_CA : command :=
-  CheckNonce (rand r) r ;;    (* 12 *)
-  MakeCert pubNewKey privCA.  (* 13 *)
-
-  Definition finTPM_CA : state := 
-  sign (certificate pubNewKey) privCA ::
-  midTPM_CA.
-
-  Definition fin_CA : state := 
-  sign (certificate pubNewKey) privCA ::
-  send (rand r) ++
-  mid_CA.
+(* Protocol steps of CA *)
+(* The CA waits to recieve a message from the OEM. *)
+(* That message must be in a specific form to be considered a proper request. *)
+(* The CA will then execute its protocol steps on the input message. *)
+(* If the protocol succeeds the CA will issue a challenge [encryptedCredential (hash (publicKey k)) nonce k0] to the OEM. *)
+  Definition steps_CA (msg : message) (ident : identifier) (ek iak : pubKey) (cert : signedCert) : Prop :=
+    match msg with
+    | (pair (TCG_CSR_IDevID (Device_info id) (Cert k0 id0 k_ca') k) (signature m k')) =>
+          ident = (Device_info id) /\ ek = k0 /\ iak = k /\ cert = (Cert k0 id0 k_ca') /\
+          seq_execute (iniTPM_CA, inferFrom msg ++ ini_CA)
+                      (CheckHash 
+                          m 
+                          (TCG_CSR_IDevID (Device_info id) (Cert k0 id0 k_ca') k) ;;
+                      CheckSig 
+                          (signature m k') 
+                          k ;;
+                      CheckCert 
+                          (Cert k0 id0 k_ca') 
+                          pubTM ;;
+                      CheckAttributes 
+                          k 
+                          Restricting Signing NonDecrypting Fixing ;;
+                      TPM2_Hash 
+                          (publicKey k);;
+                      TPM2_MakeCredential 
+                          (hash (publicKey k))
+                          nonce
+                          k0 ;;
+                      Done)
+                     (hash (publicKey k) :: iniTPM_CA, 
+                        encryptedCredential (hash (publicKey k)) nonce k0 :: hash (publicKey k) :: inferFrom msg ++ ini_CA)
+    | _ => False
+    end.
 
 
-(* Protocol specification *)
-Axiom CertIAK_spec :
-  execute (iniTPM, ini) c1 (midTPM, mid) /\     (* Steps 0 - 3 *)
-  In (TCG_CSR_IDevID certEK pubNewKey) mid /\   (* Step 4 *)
-  In (sign (hash (TCG_CSR_IDevID certEK pubNewKey)) privNewKey) mid /\  (* Step 4 *)
-  execute (iniTPM_CA, send ((TCG_CSR_IDevID certEK pubNewKey),, sign (hash (TCG_CSR_IDevID certEK pubNewKey)) privNewKey) ++ ini_CA)
-           c1_CA                                (* Steps 5 - 8*)
-          (midTPM_CA, mid_CA) /\ 
-  In (encrypt (credential (hash (publicKey pubNewKey)) r) pubEK) mid_CA /\  (* Step 9 *)
-  execute (midTPM, send (encrypt (credential (hash (publicKey pubNewKey)) r) pubEK) ++ mid) 
-           c2                                   (* Step 10 *)
-          (finTPM, fin) /\
-  In (rand r) fin /\  (* Step 11 *)
-  execute (midTPM_CA, send (rand r) ++ mid_CA)
-           c2_CA                                (* Step 12 - 13 *)
-          (finTPM_CA, fin_CA).
+(* Correct protocol second steps of OEM *)
+(* OEM waits to recieve challenge from the CA *)
+Definition step7_OEM (msg : message) : sequence :=
+  TPM2_ActivateCredential msg privEK privIAK ;;
+  Done.
 
 
 
+(* Candidate minimal initial state of OEM *)
+  Definition iniTPM_OEM : tpm_state :=
+  [ privateKey privIAK ;
+    privateKey privEK ].
 
-(* Protocol Assurances *)
-(* ******************* *)
+  Definition ini_OEM : state :=
+  [ signedCertificate certEK ;
+    publicKey pubIAK ].
 
 
-(* A TPM is authentic *)
-(* EK Certificate is valid *)
-  Theorem authenticTPM : exists st st',
-    execute st (CheckCert certEK pubTM) st'.
+  Lemma ini_OEM_lowerBound : forall iniTPM ini midTPM mid fin,
+    seq_execute (iniTPM, ini) steps1to4_OEM (midTPM, mid) ->
+    seq_execute (midTPM, inferFrom (encryptedCredential (hash (publicKey pubIAK)) nonce pubEK) ++ mid) 
+                (step7_OEM (encryptedCredential (hash (publicKey pubIAK)) nonce pubEK))
+                fin ->
+    (iniTPM_OEM \subsetOf iniTPM) /\
+    (ini_OEM \subsetOf ini).
   Proof.
-    assert (H : execute (iniTPM_CA, send ((TCG_CSR_IDevID certEK pubNewKey),, sign (hash (TCG_CSR_IDevID certEK pubNewKey)) privNewKey) ++ ini_CA) c1_CA (midTPM_CA, mid_CA)). apply CertIAK_spec.
-    repeat (apply sequence_split in H; destruct H; destruct H).
-    eexists; eexists; apply H4.
+    intros iniTPM ini midTPM mid fin E1 E2.
+(* split steps_Owner into its individual commands *)
+    inversion E1 as [initial mid0 final command steps_Owner' H_MakeCSR E10| ]; subst;
+    inversion E10 as [initial mid1 final command steps_Owner' H_Hash E11| ]; subst;
+    inversion E11 as [initial mid2 final command steps_Owner' H_Sign E12| ]; subst;
+    inversion E12 as [initial mid3 final command steps_Owner' H_MakePair E13| ]; subst;
+    inversion E13; subst;
+(* Invert each individual step in reverse order *)
+    inversion H_MakePair; subst; 
+    inversion H_Sign; subst;
+    inversion H_Hash; subst;
+    inversion H_MakeCSR; subst;
+    clear E1 E10 E11 E12 E13;
+    clear H_MakeCSR H_Hash H_Sign H_MakePair;
+    inversion E2 as [initial mid0 final command steps_Owner' H_ActivateCredential E20| ]; subst;
+    inversion E20; subst;
+    inversion H_ActivateCredential; subst;
+    clear E2 E20;
+    clear H_ActivateCredential;
+    split.
+    - unfold iniTPM_OEM; intros m I; inversion I; subst.
+    -- rewrite <- H14. inversion H17 as [EQ_false | H17']; subst.
+        inversion EQ_false.
+        assumption.
+    -- inversion H; subst. rewrite <- H12. inversion H16 as [EQ_false | H16']; subst.
+        inversion EQ_false.
+        assumption.
+        inversion H1.
+    - unfold ini_OEM; intros m I; inversion I; subst.
+    -- assumption.
+    -- inversion H; subst. assumption.
+       inversion H1.
+    - unfold iniTPM_OEM; intros m I; inversion I; subst.
+    -- rewrite <- H14. inversion H17 as [EQ_false | H17']; subst.
+        inversion EQ_false.
+        assumption.
+    -- inversion H; subst. rewrite <- H12. inversion H16 as [EQ_false | H16']; subst.
+        inversion EQ_false.
+        assumption.
+        inversion H1.
+    - unfold ini_OEM; intros m I; inversion I; subst.
+    -- assumption.
+    -- inversion H; subst. assumption. inversion H1.
   Qed.
 
 
-(* This specific TPM is authentic and is represented by the EK Certificate *)
-(* EK resident in this TPM corresponds to the EK Certificate *)
-  Theorem authenticThisTPM : 
-    certEK = sign (certificate pubEK) (pubtoPrivKey pubTM).
+
+  Lemma ini_OEM_sufficient : forall msg,
+    endorsementKey pubEK ->
+    steps_CA msg (Device_info devInfo) pubEK pubIAK certEK ->
+    exists midTPM mid fin, 
+    seq_execute (iniTPM_OEM, ini_OEM) steps1to4_OEM (midTPM, mid) /\
+    seq_execute (midTPM, inferFrom (encryptedCredential (hash (publicKey pubIAK)) nonce pubEK) ++ mid) 
+                (step7_OEM (encryptedCredential (hash (publicKey pubIAK)) nonce pubEK)) fin.
   Proof.
-(* 
-  Since the CA executed "CheckCert cerEK pubTM", 
-  we know that "certEK" must be in the form "sign (certificate k) pubTM" for some "k : pubKey". 
-*)
-    assert (H_CheckCert : exists st st', execute st (CheckCert certEK pubTM) st'). apply authenticTPM.
-    destruct H_CheckCert as [ini H_CheckCert]. destruct H_CheckCert as [fin H_CheckCert].
-    inversion H_CheckCert. subst. simpl. 
-    assert (H_certEK : sign (certificate k) (Private i r0 s d) = certEK). assumption. clear H H0 H2 H4.
-(* 
-  Since the CA executed "TPM2_MakeCredential (hash (publicKey pubNewKey)) r pubEK)", 
-  we know that "pubEK" must have the "Decrypting" attribute
-  and "pubEK" must be in the CA's state.
-*)
-    assert (H : execute (iniTPM_CA, send ((TCG_CSR_IDevID certEK pubNewKey),, sign (hash (TCG_CSR_IDevID certEK pubNewKey)) privNewKey) ++ ini_CA) c1_CA (midTPM_CA, mid_CA)). apply CertIAK_spec.
-    repeat (apply sequence_split in H; destruct H; destruct H).
-    inversion H0. subst.
-(*
-  Since "pubEK" must be in the CA's state,
-  we can show that "pubEK" must be discoverable from the sent "certEK"
-  and hence "k" is "pubEK".
-*)
-    rewrite <- H_certEK in H16. unfold ini_CA in H16. simpl in H16.
-    destruct H16 as [H16|H16]. inversion H16.
-    destruct H16 as [H16|H16]. inversion H16.
-    destruct H16 as [H16|H16]. inversion H16.
-    destruct H16 as [H16|H16]. inversion H16.
-    destruct H16 as [H16|H16]. inversion H3. subst. rewrite <- H9 in H16. inversion H16.
-    destruct H16 as [H16|H16]. inversion H16.
-    destruct H16 as [H16|H16]. inversion H16.
-    destruct H16 as [H16|H16]. inversion H16. reflexivity.
-    destruct H16 as [H16|H16]. inversion H16.
-    destruct H16 as [H16|H16]. inversion H16.
-    destruct H16 as [H16|H16]. inversion H16. rewrite H8 in H7. symmetry in H7. apply DistinctKeys in H7. inversion H7.
-    destruct H16 as [H16|H16]. inversion H16.
-    destruct H16 as [H16|H16]. inversion H16. rewrite H8 in H7. symmetry in H7. apply DistinctKeys in H7. inversion H7.
-    inversion H16.
+    intros m goodEK CA.
+    unfold iniTPM_OEM, ini_OEM, steps1to4_OEM, step7_OEM, privEK, privIAK.
+    destruct pubEK, r, s, d, f; simpl in goodEK; try inversion goodEK.
+    destruct m; try inversion CA;
+    destruct m1; try inversion CA;
+    destruct i; try inversion CA;
+    destruct s; try inversion CA;
+    destruct m2; try inversion CA; subst.
+    destruct H0; subst; destruct H1; subst; destruct H1; subst.
+    clear CA; simpl in *.
+    inversion H1 as [initial mid1 final command steps_Owner' H_CheckHash H11 | ]; subst; 
+    inversion H11 as [initial mid2 final command steps_Owner' H_CheckSig H12 | ]; subst;
+    inversion H12 as [initial mid3 final command steps_Owner' H_CheckCert H13 | ]; subst;
+    inversion H13 as [initial mid4 final command steps_Owner' H_CheckAttributes H14 | ]; subst;
+    inversion H14 as [initial mid5 final command steps_Owner' H_Hash H15 | ]; subst;
+    inversion H15 as [initial mid6 final command steps_Owner' H_MakeCredential H16 | ]; subst;
+    inversion H16; subst.
+    inversion H_MakeCredential; subst;
+    inversion H_Hash; subst;
+    inversion H_CheckAttributes; subst.
+    eexists. eexists. eexists. 
+    split. repeat eapply SE_Seq; econstructor; simpl; auto.
+    
+    eapply SE_Seq. econstructor; simpl; auto.
+    econstructor; simpl; auto 9. econstructor.
   Qed.
 
 
-(* This AK is authentic *)
-(* AK in CSR is resident in the same TPM as the EK *)
-  Theorem authenticThisAK :
-    In (privateKey privNewKey) finTPM /\
-    In (privateKey privEK) finTPM.
+
+  Lemma ca_implies_isSuperseqOfSteps1to4 : forall s iniTPM ini midTPM mid msg ident ek iak cert,
+    seq_execute (iniTPM, ini) s (midTPM, mid) ->
+    In msg mid ->
+    (forall m', needsGeneratedTPM m' -> ~ In m' iniTPM) ->
+    (forall m', needsGenerated m' -> ~ In m' ini) ->
+    steps_CA msg ident ek iak cert -> 
+    isSuperseqOfSteps1to4_OEM s ident cert iak.
   Proof.
-    unfold finTPM; unfold midTPM; unfold iniTPM;
-    split; simpl; auto 9.
+    intros s iniTPM ini finTPM fin m ident ek iak cert E I N_TPM N CA.
+(* Get m into the form of the match statement in steps_CA *)
+    destruct m; try inversion CA;
+    destruct m1; try inversion CA;
+    destruct i; try inversion CA;
+    destruct s0; try inversion CA;
+    destruct m2; try inversion CA; subst;
+    destruct H0; subst; destruct H0; subst; destruct H0; subst;
+    clear CA; simpl in *.
+(* Split steps_CA into its individual commands *)
+    inversion H0 as [initial mid1 final command steps_Owner' H_CheckHash H1 | ]; subst; 
+    inversion H1 as [initial mid2 final command steps_Owner' H_CheckSig H2 | ]; subst;
+    inversion H2 as [initial mid4 final command steps_Owner' H_CheckCert H3 | ]; subst;
+    inversion H3 as [initial mid5 final command steps_Owner' H_CheckAttributes H4 | ]; subst;
+    inversion H4; subst;
+(* Invert each individual step in reverse order *) 
+    inversion H_CheckAttributes; subst;
+    inversion H_CheckCert; subst;
+    inversion H_CheckSig; subst;
+    inversion H_CheckHash; subst.
+(* Apply lemma *)
+    eapply isSuperseqOfSteps1to4_OEM_lemma; eauto; 
+    try apply N; try apply N_TPM; simpl; trivial.
   Qed.
 
 
-(* This AK is in fact an AK *)
-  Theorem pubNewKey_AK :
-    attestationKey pubNewKey.
+
+
+
+
+  
+  Lemma rand_implies_isSuperseqOfStep7 : forall s2 midTPM mid finTPM fin ek iak g,  
+    seq_execute (midTPM, mid) s2 (finTPM, fin) ->
+    In (encryptedCredential (hash (publicKey iak)) g ek) mid ->
+    (forall ki ke, iak <> ki -> ~(In (encryptedCredential (hash (publicKey ki)) g ke) mid)) ->
+    (forall ki ke, ek <> ke -> ~(In (encryptedCredential (hash (publicKey ki)) g ke) mid)) ->
+    ~ (In (randomNum g)) mid ->
+    In (randomNum g) fin ->
+    isSuperseqOfStep7_OEM s2 ek iak g.
   Proof.
-    assert (H : execute (iniTPM_CA, send ((TCG_CSR_IDevID certEK pubNewKey),, sign (hash (TCG_CSR_IDevID certEK pubNewKey)) privNewKey) ++ ini_CA) c1_CA (midTPM_CA, mid_CA)). apply CertIAK_spec.
-    repeat (apply sequence_split in H; destruct H; destruct H).
-    inversion H3. subst. simpl. trivial.
+    induction s2; intros midTPM mid finTPM fin ek iak g E Im N_IAK N_EK N I.
+    - destruct c; simpl in *; inversion E; inversion H2;
+      subst; try (eapply IHs2; fdeq);
+      try (eapply IHs2; 
+      [ eauto 
+      | simpl 
+      | intros ki ke Neq HC; inversion HC; try inversion H; try congruence; destruct (N_IAK ki ke); assumption
+      | intros ki ke Neq HC; inversion HC; try inversion H; try congruence; destruct (N_EK ki ke); assumption
+      | fdeq |  ]; eauto).
+      destruct n; inversion H14.
+      destruct (decEq g g0);
+      destruct (decEq ek (Public i r s0 d f));
+      destruct (decEq iak (Public i0 r0 s1 d0 f0));
+      destruct (decEq (pubToPrivKey ek) (Private i r s0 d f));
+      destruct (decEq (pubToPrivKey iak) (Private i0 r0 s1 d0 f0)); subst; trivial;
+      eapply IHs2; eauto; try (simpl; eauto; fail); 
+      try (intros ki ke Neq HC; inversion HC; try inversion H; destruct (N_IAK ki ke); assumption); 
+      try (intros ki ke Neq HC; inversion HC; try inversion H; destruct (N_EK ki ke); assumption);
+      try (destruct (N_IAK (Public i0 r0 s1 d0 f0) (Public i r s0 d f)); assumption);
+      try (destruct (N_EK (Public i0 r0 s1 d0 f0) (Public i r s0 d f)); assumption);
+      try (intros HC; inversion HC; congruence).
+    - inversion E; subst; congruence.
   Qed.
+
+  
+
+
+
+  Lemma ca_and_rand_implies_isSuperseqOfStep7 : forall s2 s1 iniTPM ini midTPM mid finTPM fin msg ident ek iak cert g,
+    seq_execute (iniTPM, ini) s1 (midTPM, mid) -> 
+    In msg mid ->
+    (forall m', needsGeneratedTPM m' -> ~ In m' iniTPM) ->
+    (forall m', needsGenerated m' -> ~ In m' ini) ->
+    steps_CA msg ident ek iak cert ->
+    seq_execute (midTPM, inferFrom (encryptedCredential (hash (publicKey iak)) g ek) ++ mid) 
+                 s2 
+                (finTPM, fin) ->
+    In (randomNum g) fin ->
+    isSuperseqOfStep7_OEM s2 ek iak g.
+  Proof.
+    intros s2 s1 iniTPM ini midTPM mid finTPM fin m ident ek iak cert g.
+    intros E1 Im N_TPM N CA E2 Ig.
+
+    destruct m; try inversion CA;
+    destruct m1; try inversion CA;
+    destruct i; try inversion CA;
+    destruct s; try inversion CA;
+    destruct m2; try inversion CA; subst;
+    destruct H0; subst; destruct H0; subst; destruct H0; subst;
+    clear CA; simpl in *.
+
+    inversion H0 as [initial mid1 final command steps_Owner' H_CheckHash H1 | ]; subst; 
+    inversion H1 as [initial mid2 final command steps_Owner' H_CheckSig H2 | ]; subst;
+    inversion H2 as [initial mid4 final command steps_Owner' H_CheckCert H3 | ]; subst;
+    inversion H3 as [initial mid5 final command steps_Owner' H_CheckAttributes H4 | ]; subst;
+    inversion H4; subst.
+
+    inversion H_CheckAttributes; subst;
+    inversion H_CheckCert; subst;
+    inversion H_CheckSig; subst;
+    inversion H_CheckHash; subst.
+
+    eapply rand_implies_isSuperseqOfStep7. eauto.
+    simpl; eauto.
+
+    intros ki ke Neq HC. inversion HC; subst. inversion H. congruence.
+    assert (contra : ~ In (encryptedCredential (hash (publicKey ki)) g ke) mid).
+    eapply seq_exec_cannotGenerateCred_contrapositive; eauto. 
+    intros n k HCC; destruct (N (encryptedCredential n g k)); simpl; trivial.
+    intros HCC; destruct (N (randomNum g)); simpl; trivial.
+    congruence.
+
+    intros ki ke Neq HC. inversion HC; subst. inversion H. congruence.
+    assert (contra : ~ In (encryptedCredential (hash (publicKey ki)) g ke) mid).
+    eapply seq_exec_cannotGenerateCred_contrapositive; eauto. 
+    intros n k HCC; destruct (N (encryptedCredential n g k)); simpl; trivial.
+    intros HCC; destruct (N (randomNum g)); simpl; trivial.
+    congruence.
+
+    intros HC. inversion HC; try inversion H. clear HC. generalize dependent H.
+    eapply seq_exec_cannotGenerateRand_contrapositive; eauto.
+    intros HC; destruct (N (randomNum g)); simpl; trivial.
+    intros n k HC; destruct (N (encryptedCredential n g k)); simpl; trivial.
+
+    assumption.
+  Qed.
+
+
+  Lemma isSuperseqOfStep7_implies_activatecredential : forall s2 ek iak g,
+    isSuperseqOfStep7_OEM s2 ek iak g ->
+    command_in_sequence (TPM2_ActivateCredential (encryptedCredential (hash (publicKey iak)) g ek) 
+                                                (pubToPrivKey ek) 
+                                                (pubToPrivKey iak))
+                        s2.
+  Proof.
+    induction s2; intros ek iak g H0; simpl.
+    - destruct (decEq 
+                  (TPM2_ActivateCredential (encryptedCredential (hash (publicKey iak)) g ek)
+                                           (pubToPrivKey ek) 
+                                           (pubToPrivKey iak)) 
+                   c);
+      [ trivial
+      | apply IHs2; simpl in *;
+        destruct c; try assumption;
+        destruct m; subst; try assumption; 
+        destruct m; subst; try assumption; 
+        destruct m; subst; try assumption;        
+        destruct (decEq g r);
+        destruct (decEq ek p1);
+        destruct (decEq iak p2);
+        destruct (decEq (pubToPrivKey ek) p);
+        destruct (decEq (pubToPrivKey iak) p0); 
+        subst; congruence ].
+    - inversion H0.
+  Qed.
+
+
+  Lemma activatecredential_implies_iakInTPM : forall s2 midTPM mid finTPM fin ek iak g,
+    seq_execute (midTPM, mid) s2 (finTPM, fin) -> 
+    command_in_sequence (TPM2_ActivateCredential (encryptedCredential (hash (publicKey iak)) g ek) 
+                                               (pubToPrivKey ek) 
+                                               (pubToPrivKey iak))
+                        s2 ->
+    In (privateKey (pubToPrivKey iak)) midTPM.
+  Proof.
+    induction s2; intros midTPM mid finTPM fin ek iak g E CI.
+    - simpl in *;
+      destruct (decEq 
+                  (TPM2_ActivateCredential (encryptedCredential (hash (publicKey iak)) g ek)
+                                           (pubToPrivKey ek) 
+                                           (pubToPrivKey iak)) 
+                   c);
+      inversion E; subst.
+    -- inversion H2; assumption.
+    -- destruct mid0 as [midTPM0 mid0]; eapply exec_cannotGenerateKey; eauto.
+    - inversion CI.
+  Qed.
+
+
+  Lemma activatecredential_implies_ekInTPM : forall s2 midTPM mid finTPM fin ek iak g,
+    seq_execute (midTPM, mid) s2 (finTPM, fin) -> 
+    command_in_sequence (TPM2_ActivateCredential (encryptedCredential (hash (publicKey iak)) g ek) 
+                                               (pubToPrivKey ek) 
+                                               (pubToPrivKey iak)) 
+                      s2->
+    In (privateKey (pubToPrivKey ek)) midTPM.
+  Proof.
+    induction s2; intros midTPM mid finTPM fin ek iak g E CI.
+    - simpl in *;
+      destruct (decEq 
+                  (TPM2_ActivateCredential (encryptedCredential (hash (publicKey iak)) g ek)
+                                           (pubToPrivKey ek) 
+                                           (pubToPrivKey iak)) 
+                  c);
+      inversion E; subst.
+    -- inversion H2; assumption.
+    -- destruct mid0 as [midTPM0 mid0]; eapply exec_cannotGenerateKey; eauto.
+    - inversion CI.
+  Qed.
+
+
+(* PROTOCOL ASSURANCES *)
+(* Given the following assumptions: 
+      The OEM executes some sequence of steps
+      resulting in a message in its intermediate final state
+      when only keys and certificates may be in its initial states.
+      The CA's protocol executes successfully on the given message.
+      The OEM executes some other sequence of steps upon receiving the CA's challenge
+      resulting in the nonce in its final state.
+*)
+
+(* Conclude:
+      The private EK and private IAK reside in the same TPM *)
+  Theorem iak_and_ek_in_TPM : forall s2 s1 iniTPM ini midTPM mid finTPM fin msg ident ek iak cert g,
+    seq_execute (iniTPM, ini) s1 (midTPM, mid) -> 
+    In msg mid ->
+    (forall m', needsGeneratedTPM m' -> ~ In m' iniTPM) ->
+    (forall m', needsGenerated m' -> ~ In m' ini) ->
+    steps_CA msg ident ek iak cert ->
+    seq_execute (midTPM, inferFrom (encryptedCredential (hash (publicKey iak)) g ek) ++ mid) 
+                 s2 
+                (finTPM, fin) ->
+    In (randomNum g) fin ->
+    In (privateKey (pubToPrivKey iak)) iniTPM /\ In (privateKey (pubToPrivKey ek)) iniTPM.
+  Proof.
+    intros s2 s1 iniTPM ini midTPM mid finTPM fin m ident ek iak cert g;
+    intros E1 Im N_TPM N CA E2 Ig;
+    split; eapply seq_exec_cannotGenerateKey; eauto; 
+    [ eapply activatecredential_implies_iakInTPM | eapply activatecredential_implies_ekInTPM ]; eauto;
+    eapply isSuperseqOfStep7_implies_activatecredential; eapply ca_and_rand_implies_isSuperseqOfStep7 with (s1 := s1); eauto.
+  Qed.
+
+
+(* Conclude:
+      The EK certificate is valid and signed by the TPM Manufacturer *)
+  Theorem ek_certificate_valid : forall msg ident ek iak cert,
+    steps_CA msg ident ek iak cert ->
+    execute (iniTPM_CA, inferFrom msg ++ ini_CA) 
+            (CheckCert cert pubTM) 
+            (iniTPM_CA, inferFrom msg ++ ini_CA).
+  Proof.
+    intros m ident ek iak cert CA.
+
+    destruct m; try inversion CA;
+    destruct m1; try inversion CA;
+    destruct i; try inversion CA;
+    destruct s; try inversion CA;
+    destruct m2; try inversion CA; subst;
+    destruct H0; subst; destruct H0; subst; destruct H0; subst;
+    clear CA; simpl in *.
+
+    inversion H0 as [initial mid1 final command steps_Owner' H_CheckHash H1 | ]; subst; 
+    inversion H1 as [initial mid2 final command steps_Owner' H_CheckSig H2 | ]; subst;
+    inversion H2 as [initial mid4 final command steps_Owner' H_CheckCert H3 | ]; subst;
+    inversion H3 as [initial mid5 final command steps_Owner' H_CheckAttributes H4 | ]; subst;
+    inversion H4; subst.
+
+    inversion H_CheckAttributes; subst;
+    inversion H_CheckCert; subst;
+    inversion H_CheckSig; subst;
+    inversion H_CheckHash; subst.
+
+    constructor; simpl; auto.
+  Qed.
+
+(* Conclude:
+      The IAK is a Restricted Signing NonDecrypting key *)
+  Theorem iak_good_attributes : forall msg ident ek iak cert,
+    steps_CA msg ident ek iak cert ->
+    attestationKey iak.
+  Proof.
+    intros m ident ek iak cert CA;
+    destruct m; try inversion CA;
+    destruct m1; try inversion CA;
+    destruct i; try inversion CA;
+    destruct s; try inversion CA;
+    destruct m2; try inversion CA; subst;
+    destruct H0; subst; destruct H0; subst; destruct H0; subst;
+    clear CA; simpl in *.
+    inversion H0 as [initial mid1 final command steps_Owner' H_CheckHash H1 | ]; subst; 
+    inversion H1 as [initial mid2 final command steps_Owner' H_CheckSig H2 | ]; subst;
+    inversion H2 as [initial mid4 final command steps_Owner' H_CheckCert H3 | ]; subst;
+    inversion H3 as [initial mid5 final command steps_Owner' H_CheckAttributes H4 | ]; subst;
+    inversion H4; subst.
+    inversion H_CheckAttributes; subst;
+    simpl; trivial.
+  Qed.
+
+(* Prove command_in_sequence s1 (TPM2_Sign _ (pubToPrivKey iak)) to show that OEM has control of the key *)
+
 
 End IAK_Cert_Protocol.
 
 
 
+(*
 
-
-
-
-
-
-
-
-
-
-
-
-Module myIAK <: IAK_Cert_Protocol.
+Module goodIAK <: IAK_Cert_Protocol.
 
 (* OEM parameters *)
-  Definition pubNewKey : pubKey := Public 11 Restricted Signing NonDecrypting.
-  Definition privNewKey : privKey := Private 11 Restricted Signing NonDecrypting.
-  Definition pubEK : pubKey := Public 10 Restricted NonSigning Decrypting.
-  Definition privEK : privKey := Private 10 Restricted NonSigning Decrypting.
-  Definition certEK : message := sign (certificate (Public 10 Restricted NonSigning Decrypting)) 
-                                      (Private 0 NonRestricted Signing NonDecrypting).
+  Definition pubNewKey : pubKey := Public 51 Restricting Signing NonDecrypting.
+  Definition pubEK : pubKey := Public 50 Restricting NonSigning Decrypting.
+  Definition certEK : signedCert := Cert (Public 50 Restricting NonSigning Decrypting) (TPM_info 555) (Private 0 NonRestricting Signing NonDecrypting).
+  Definition devInfo : deviceInfoType := 5.
 
 (* CA parameters *)
-  Definition pubCA : pubKey := Public 1 NonRestricted Signing NonDecrypting.
-  Definition privCA : privKey := Private 1 NonRestricted Signing NonDecrypting.
-  Definition pubTM : pubKey := Public 0 NonRestricted Signing NonDecrypting.
-  Definition r : randType := 5.
-
-  Local Hint Unfold pubNewKey privNewKey pubEK privEK certEK : core.
-  Local Hint Unfold pubCA privCA pubTM r : core.
+  Definition pubCA : pubKey := Public 1 NonRestricting Signing NonDecrypting.
+  Definition privCA : privKey := Private 1 NonRestricting Signing NonDecrypting.
+  Definition pubTM : pubKey := Public 0 NonRestricting Signing NonDecrypting.
+  Definition g : randType := 11.
 
 
-  Theorem DistinctKeys :
+
+  Theorem keys_distinct :
     pubNewKey <> pubEK /\
     pubNewKey <> pubCA /\
     pubNewKey <> pubTM /\
@@ -872,181 +2419,123 @@ Module myIAK <: IAK_Cert_Protocol.
     pubEK <> pubTM /\
     pubCA <> pubTM.
   Proof.
-    repeat split; intros H; inversion H.
+    repeat split; intros contra; inversion contra.
   Qed.
 
 
-  Definition iniTPM : tpm_state :=
-  [ publicKey pubNewKey ;
-  privateKey privNewKey ;
-  publicKey pubEK ;
-  privateKey privEK ].
-
-  Definition ini : state :=
-  [ publicKey pubNewKey ;
-  privateKey privNewKey ;
-  certEK ;    (* EK certificate *)
-  publicKey pubEK ;
-  privateKey privEK ].
+Definition privIAK := pubToPrivKey pubNewKey.
+Definition privEK := pubToPrivKey pubEK.
 
 
-  Definition c1 : command :=
-  MakeCSR_IDevID certEK pubNewKey ;;                              (* 1 *)
-  TPM2_Hash (TCG_CSR_IDevID certEK pubNewKey) ;;                  (* 2 *)
-  TPM2_Sign (hash (TCG_CSR_IDevID certEK pubNewKey)) privNewKey.  (* 3 *)
+Definition min_iniTPM_OEM : tpm_state :=
+[ privateKey privIAK ].
+
+Definition min_ini_OEM : state :=
+[ publicKey pubNewKey ;
+  signedCertificate certEK ].
 
 
-  Definition midTPM : state :=
-  sign (hash (TCG_CSR_IDevID certEK pubNewKey)) privNewKey ::
-  hash (TCG_CSR_IDevID certEK pubNewKey) ::
-  iniTPM.
 
-  Definition mid : state :=
-  sign (hash (TCG_CSR_IDevID certEK pubNewKey)) privNewKey ::
-  hash (TCG_CSR_IDevID certEK pubNewKey) ::
-  (TCG_CSR_IDevID certEK pubNewKey) ::
-  ini.
+Definition steps1_OEM : sequence :=
+  MakeCSR_IDevID (Device_info devInfo) certEK pubNewKey ;;
+  TPM2_Hash (TCG_CSR_IDevID (Device_info devInfo) certEK pubNewKey) ;;
+  TPM2_Sign (hash (TCG_CSR_IDevID (Device_info devInfo) certEK pubNewKey)) privIAK ;;
+  MakePair (TCG_CSR_IDevID (Device_info devInfo) certEK pubNewKey)
+           (signature (hash (TCG_CSR_IDevID (Device_info devInfo) certEK pubNewKey)) privIAK) ;;
+  Done.
 
-  Local Hint Unfold mid midTPM c1 ini iniTPM : core.
 
-(*
-  send ((TCG_CSR_IDevID certEK pubNewKey),, (sign (hash (TCG_CSR_IDevID certEK pubNewKey)) privNewKey))   (* 4 *)
-*)
+Theorem steps1_lowerBound : forall iniTPM ini fin,
+  seq_execute (iniTPM, ini) steps1_OEM fin ->
+  (min_iniTPM_OEM \subsetOf iniTPM) /\
+  (min_ini_OEM \subsetOf ini).
+Proof.
+  intros iniTPM ini fin E.
 
-  Definition iniTPM_CA : tpm_state :=
+  inversion E as [initial mid1 final command steps_Owner' H_MakeCSR E0| ]; subst. 
+  inversion E0 as [initial mid2 final command steps_Owner' H_Hash E1| ]; subst.
+  inversion E1 as [initial mid3 final command steps_Owner' H_Sign E2| ]; subst.
+  inversion E2 as [initial mid4 final command steps_Owner' H_MakePair E3| ]; subst.
+  inversion E2; subst.
+  inversion E_MakePair; subst; 
+  inversion E_Sign; subst;
+  inversion E_Hash; subst;
+  inversion E_MakeCSR; subst;
+  clear E E' E'' E''' E'''';
+  clear E_MakeCSR E_Hash E_Sign E_MakePair;
+  split.
+
+  - unfold min_iniTPM_OEM; intros m I; inversion I; subst.
+  -- unfold privIAK; simpl ; inversion H3 as [EQ_false | H3']; subst.
+      inversion EQ_false.
+      assumption.
+  -- inversion H; subst.
+
+  - unfold min_ini_OEM; intros m I; inversion I; subst.
+  -- assumption.
+  -- inversion H; subst.
+  --- assumption.
+  --- inversion H0.
+Qed.
+
+
+
+
+Theorem steps1_min : exists fin,
+  seq_execute (min_iniTPM_OEM, min_ini_OEM) steps1_OEM fin.
+Proof.
+  eexists; unfold min_iniTPM_OEM; unfold min_ini_OEM; unfold steps1_OEM;
+  unfold privIAK; unfold privEK; unfold certEK;
+  unfold pubNewKey; unfold pubEK.
+  repeat eapply E_Seq; constructor; simpl; auto.
+Qed.
+
+
+
+Definition iniTPM_CA : tpm_state :=
   [ privateKey privCA ;
-  publicKey pubCA ].
+    publicKey pubCA ].
 
   Definition ini_CA : state :=
   [ publicKey pubTM ;
-  privateKey privCA ;
-  publicKey pubCA ].
+    privateKey privCA ;
+    publicKey pubCA ].
+
+  Theorem CA_keys_good :
+    privCA = pubToPrivKey pubCA /\
+    caKey pubCA /\
+    caKey pubTM.
+  Proof.
+    repeat split.
+  Qed.
 
 
-  Definition c1_CA : command :=
-  CheckHash (hash (TCG_CSR_IDevID certEK pubNewKey)) (TCG_CSR_IDevID certEK pubNewKey) ;; (* 5a *)
-  CheckSig (sign (hash (TCG_CSR_IDevID certEK pubNewKey)) privNewKey) pubNewKey ;;        (* 5b *)
-  CheckCert certEK pubTM ;;                                                               (* 5c *)
-  CheckAttributes pubNewKey Restricted Signing NonDecrypting ;;                           (* 5d *)
-  TPM2_Hash (publicKey pubNewKey) ;;                                                      (* 6 *)
-  TPM2_GetRandom r ;;                                                                     (* 7 *)
-  TPM2_MakeCredential (hash (publicKey pubNewKey)) r pubEK.                               (* 8 *)
+
+  Definition steps_CA (m : message) : Prop :=
+    match m with
+    | ((TCG_CSR_IDevID (Device_info id) (Cert k_EK id0 k_ca') k),,
+       (signature m k')) =>
+          seq_execute (iniTPM_CA, inferFrom m ++ ini_CA)
+                            (CheckHash m 
+                                      (TCG_CSR_IDevID (Device_info id) (Cert k_EK id0 k_ca') k) ;;
+                            CheckSig (signature m k') k ;;
+                            CheckCert (Cert k_EK id0 k_ca') pubTM ;;
+                            CheckAttributes k Restricting Signing NonDecrypting ;;
+                            TPM2_Hash (publicKey k) ;;
+                            TPM2_MakeCredential (hash (publicKey k)) g k_EK ;;
+                            Done)
+                            (iniTPM_CA, 
+                             inferFrom m ++ ini_CA)
+    | _ => False
+    end.
 
 
-  Definition midTPM_CA : tpm_state :=
-  encrypt (credential (hash (publicKey pubNewKey)) r) pubEK ::
-  rand r ::
-  hash (publicKey pubNewKey) ::
-  iniTPM_CA.
+(* Correct protocol second steps of OEM *)
+(* OEM waits to recieve challenge from the CA *)
+  Definition steps2_OEM (m : message) : sequence :=
+    TPM2_ActivateCredential m privEK privIAK ;;
+    Done.
 
-  Definition mid_CA : state :=
-  encrypt (credential (hash (publicKey pubNewKey)) r) pubEK ::
-  rand r ::
-  hash (publicKey pubNewKey) ::
-  send ((TCG_CSR_IDevID certEK pubNewKey),, (sign (hash (TCG_CSR_IDevID certEK pubNewKey)) privNewKey)) ++
-  ini_CA.
+End goodIAK.
 
-  Local Hint Unfold mid_CA midTPM_CA c1_CA ini_CA iniTPM_CA : core.
-
-(*
-  send (encrypt (credential (hash (publicKey pubNewKey)) r) pubEK)    (* 9 *)
 *)
-
-  Definition c2 : command :=
-  TPM2_ActivateCredential (encrypt (credential (hash (publicKey pubNewKey)) r) pubEK) privEK (privNewKey).  (* 10 *)
-
-
-  Definition finTPM : tpm_state :=
-  rand r ::
-  credential (hash (publicKey pubNewKey)) r ::
-  midTPM.
-
-  Definition fin : state :=
-  rand r ::
-  credential (hash (publicKey pubNewKey)) r  ::
-  send (encrypt (credential (hash (publicKey pubNewKey)) r) pubEK) ++
-  mid.
-
-  Local Hint Unfold fin finTPM c2 : core.
-
-(*
-  send (rand r)    (* 11 *)
-*)
-
-  Definition c2_CA : command :=
-  CheckNonce (rand r) r ;;    (* 12 *)
-  MakeCert pubNewKey privCA.  (* 13 *)
-
-  Definition finTPM_CA : state := 
-  sign (certificate pubNewKey) privCA ::
-  midTPM_CA.
-
-  Definition fin_CA : state := 
-  sign (certificate pubNewKey) privCA ::
-  send (rand r) ++
-  mid_CA.
-
-  Local Hint Unfold fin_CA finTPM_CA c2_CA : core.
-
-(* Protocol execution *)
-  Theorem CertIAK_spec :
-    execute (iniTPM, ini) c1 (midTPM, mid) /\     (* Steps 0 - 3 *)
-    In (TCG_CSR_IDevID certEK pubNewKey) mid /\   (* Step 4 *)
-    In (sign (hash (TCG_CSR_IDevID certEK pubNewKey)) privNewKey) mid /\  (* Step 4 *)
-    execute (iniTPM_CA, send ((TCG_CSR_IDevID certEK pubNewKey),, sign (hash (TCG_CSR_IDevID certEK pubNewKey)) privNewKey) ++ ini_CA)
-           c1_CA                                (* Steps 5 - 8*)
-          (midTPM_CA, mid_CA) /\ 
-    In (encrypt (credential (hash (publicKey pubNewKey)) r) pubEK) mid_CA /\  (* Step 9 *)
-    execute (midTPM, send (encrypt (credential (hash (publicKey pubNewKey)) r) pubEK) ++ mid) 
-           c2                                   (* Step 10 *)
-          (finTPM, fin) /\
-    In (rand r) fin /\  (* Step 11 *)
-    execute (midTPM_CA, send (rand r) ++ mid_CA)
-           c2_CA                                (* Step 12 - 13 *)
-          (finTPM_CA, fin_CA).
-  Proof.
-    repeat split; autounfold; repeat execute_constructor; simpl; auto 11.
-  Qed.
-
-
-
-
-(* A TPM is authentic *)
-(* EK Certificate is valid *)
-  Theorem authenticTPM : exists st st',
-    execute st (CheckCert certEK pubTM) st'.
-  Proof.
-    exists ([], [certEK; publicKey pubTM]); exists ([], [certEK; publicKey pubTM]);
-    execute_constructor; simpl; auto.
-  Qed.
-
-
-(* This specific TPM is authentic and is represented by the EK Certificate *)
-(* EK resident in this TPM corresponds to the EK Certificate *)
-  Theorem authenticThisTPM : 
-    certEK = sign (certificate pubEK) (pubtoPrivKey pubTM).
-  Proof.
-    autounfold; reflexivity.
-  Qed.
-
-
-(* This AK is authentic *)
-(* AK in CSR is resident in the same TPM as the EK *)
-  Theorem authenticThisAK :
-    In (privateKey privNewKey) finTPM /\
-    In (privateKey privEK) finTPM.
-  Proof.
-    autounfold; simpl; auto 10.
-  Qed.
-
-
-(* This AK is in fact an AK *)
-  Theorem pubNewKey_AK :
-    attestationKey pubNewKey.
-  Proof.
-    autounfold; simpl; trivial.
-  Qed.
-
-
-End myIAK. 
-
